matching-logic/src/ProofMode_base.v
@@ -1,0 +1,423 @@
+From Coq Require Import ssreflect ssrfun ssrbool.
+Set Implicit Arguments.
+Unset Strict Implicit.
+Unset Printing Implicit Defensive.
+
+From Ltac2 Require Import Ltac2.
+
+From Coq Require Import Ensembles Bool.
+From Coq.Logic Require Import FunctionalExtensionality Eqdep_dec.
+From Equations Require Import Equations.
+
+Require Import Coq.Program.Tactics.
+
+From MatchingLogic Require Import Syntax DerivedOperators_Syntax ProofSystem IndexManipulation wftactics.
+
+From stdpp Require Import list tactics fin_sets coGset gmap sets.
+
+From MatchingLogic.Utils Require Import stdpp_ext.
+
+Import extralibrary.
+
+Import
+  MatchingLogic.Syntax.Notations
+  MatchingLogic.DerivedOperators_Syntax.Notations
+  MatchingLogic.ProofSystem.Notations
+.
+
+Set Default Proof Mode "Classic".
+
+Open Scope ml_scope.
+
+
+
+Record MLGoal {Σ : Signature} : Type := mkMLGoal
+  { mlTheory : Theory;
+    mlHypotheses: list Pattern;
+    mlConclusion : Pattern ;
+    mlInfo : ProofSystem.ProofInfo ;
+  }.
+
+Definition MLGoal_from_goal
+  {Σ : Signature} (Γ : Theory) (goal : Pattern) (pi : ProofInfo)
+  :
+  MLGoal
+  := @mkMLGoal Σ Γ nil goal pi.
+
+Coercion of_MLGoal {Σ : Signature} (MG : MLGoal) : Type :=
+  well_formed (mlConclusion MG) ->
+  Pattern.wf (mlHypotheses MG) ->
+  (mlTheory MG) ⊢i (fold_right patt_imp (mlConclusion MG) (mlHypotheses MG))
+  using (mlInfo MG).
+
+  (* This is useful only for printing. *)
+  Notation "[ S , G ⊢ l ==> g ]  'using' pi "
+  := (@mkMLGoal S G l g pi) (at level 95, no associativity, only printing).
+
+
+Ltac toMLGoal :=
+  unfold ProofSystem.derives;
+  lazymatch goal with
+  | [ |- ?G ⊢i ?phi using ?pi]
+    => cut (of_MLGoal (MLGoal_from_goal G phi pi));
+       unfold MLGoal_from_goal;
+       [(unfold of_MLGoal; simpl; let H := fresh "H" in intros H; apply H; clear H; [|reflexivity])|]
+  end.
+
+Ltac fromMLGoal := unfold of_MLGoal; simpl; intros _ _.
+
+Ltac solve_pim_simple := constructor; simpl;[(set_solver)|(set_solver)|(reflexivity)|(apply reflexivity)].
+
+
+Lemma useBasicReasoning {Σ : Signature} (Γ : Theory) (ϕ : Pattern) (i : ProofInfo) :
+Γ ⊢i ϕ using BasicReasoning ->
+Γ ⊢i ϕ using i.
+Proof.
+intros H.
+pose proof (Hpf := proj2_sig H).
+remember (proj1_sig H) as _H.
+exists (_H).
+clear Heq_H.
+abstract (
+  destruct Hpf as [Hpf1 Hpf2 Hpf3 Hpf4];
+destruct i; constructor; simpl in *;
+[set_solver|set_solver|idtac|set_solver];
+(destruct (uses_kt _H); simpl in *; try congruence)).
+Defined.
+
+
+Lemma mlUseBasicReasoning
+  {Σ : Signature} (Γ : Theory) (l : list Pattern) (g : Pattern) (i : ProofInfo) :
+  @mkMLGoal Σ Γ l g BasicReasoning ->
+  @mkMLGoal Σ Γ l g i.
+Proof.
+  intros H wf1 wf2.
+  specialize (H wf1 wf2).
+  apply useBasicReasoning.
+  exact H.
+Defined.
+
+
+Ltac useBasicReasoning :=
+  unfold ProofSystem.derives;
+  lazymatch goal with
+  | [ |- of_MLGoal (@mkMLGoal _ _ _ _ _) ] => apply mlUseBasicReasoning
+  | [ |- _ ⊢i _ using _ ] => apply useBasicReasoning
+  end.
+
+
+(* Extracts well-formedness assumptions about (local) goal and (local) hypotheses. *)
+Tactic Notation "mlExtractWF" ident(wfl) ident(wfg) :=
+match goal with
+| [ |- ?g ] =>
+  let wfl' := fresh "wfl'" in
+  let wfg' := fresh "wfg'" in
+  intros wfg' wfl';
+  pose proof (wfl := wfl');
+  pose proof (wfg := wfg');
+  revert wfg' wfl';
+  fold g;
+  rewrite /mlConclusion in wfg;
+  rewrite /mlHypotheses in wfl
+end.
+
+Local Example ex_extractWfAssumptions {Σ : Signature} Γ (p : Pattern) :
+  well_formed p ->
+  Γ ⊢i p ---> p using BasicReasoning.
+Proof.
+  intros wfp.
+  toMLGoal.
+  { auto. }
+  mlExtractWF wfl wfg.
+  (* These two asserts by assumption only test presence of the two hypotheses *)
+  assert (Pattern.wf []) by assumption.
+  assert (well_formed (p ---> p)) by assumption.
+Abort.
+
+Lemma cast_proof' {Σ : Signature} (Γ : Theory) (ϕ ψ : Pattern) (i : ProofInfo) (e : ψ = ϕ) :
+  Γ ⊢i ϕ using i ->
+  Γ ⊢i ψ using i.
+Proof.
+  intros [pf Hpf].
+  unshelve (eexists).
+  {
+    apply (cast_proof e).
+    exact pf.
+  }
+  { abstract(
+    destruct Hpf as [Hpf2 Hpf3 Hpf4];
+    constructor; [
+    (
+      rewrite elem_of_subseteq in Hpf2;
+      rewrite elem_of_subseteq;
+      intros x Hx;
+      specialize (Hpf2 x);
+      apply Hpf2; clear Hpf2;
+      rewrite elem_of_gset_to_coGset in Hx;
+      rewrite uses_of_ex_gen_correct in Hx;
+      rewrite elem_of_gset_to_coGset;
+      rewrite uses_of_ex_gen_correct;
+      rewrite indifferent_to_cast_uses_ex_gen in Hx;
+      exact Hx
+    )|
+    (
+      rewrite elem_of_subseteq in Hpf3;
+      rewrite elem_of_subseteq;
+      intros x Hx;
+      specialize (Hpf3 x);
+      apply Hpf3; clear Hpf3;
+      rewrite elem_of_gset_to_coGset in Hx;
+      rewrite uses_of_svar_subst_correct in Hx;
+      rewrite elem_of_gset_to_coGset;
+      rewrite uses_of_svar_subst_correct;
+      rewrite indifferent_to_cast_uses_svar_subst in Hx;
+      exact Hx
+    )|
+    (
+      rewrite indifferent_to_cast_uses_kt;
+      apply Hpf4
+    )|
+    (
+      rewrite framing_patterns_cast_proof;
+      destruct i; assumption
+    )
+    ]).
+  }
+Defined.
+
+Lemma cast_proof_ml_hyps {Σ : Signature} Γ hyps hyps' (e : hyps = hyps') goal (i : ProofInfo) :
+  @mkMLGoal Σ Γ hyps goal i ->
+  @mkMLGoal Σ Γ hyps' goal i.
+Proof.
+  unfold of_MLGoal. simpl. intros H.
+  intros wfg wfhyps'.
+  feed specialize H.
+  { exact wfg. }
+  { rewrite e. exact wfhyps'. }
+  unshelve (eapply (@cast_proof' Σ Γ _ _ i _ H)).
+  rewrite e.
+  reflexivity.
+Defined.
+
+Lemma cast_proof_ml_goal {Σ : Signature} Γ hyps goal goal' (e : goal = goal') (i : ProofInfo):
+  @mkMLGoal Σ Γ hyps goal i ->
+  @mkMLGoal Σ Γ hyps goal' i .
+Proof.
+  unfold of_MLGoal. simpl. intros H.
+  intros wfgoal' wfhyps.
+  feed specialize H.
+  { rewrite e. exact wfgoal'. }
+  { exact wfhyps. }
+  unshelve (eapply (@cast_proof' Σ Γ _ _ i _ H)).
+  rewrite e.
+  reflexivity.
+Defined.
+
+Lemma cast_proof_ml_hyps_indifferent'
+      Σ P Γ hyps hyps' (e : hyps = hyps') goal (i : ProofInfo)
+      (pf : @mkMLGoal Σ Γ hyps goal i) wf1 wf2 wf3 wf4:
+  indifferent_to_cast P ->
+  P _ _ (proj1_sig (@cast_proof_ml_hyps Σ Γ hyps hyps' e goal i pf wf1 wf2)) = P _ _ (proj1_sig (pf wf3 wf4)).
+Proof.
+  intros Hp. simpl. unfold cast_proof_ml_hyps.
+  unfold proj1_sig. unfold cast_proof'. destruct pf as [pf' Hpf'] eqn:Heqpf.
+  rewrite Hp.
+  apply f_equal. simpl in *.
+  case_match. simpl in *.
+  remember (pf wf1
+  (eq_ind_r (λ pv : list Pattern, Pattern.wf pv)
+     wf2 e)).
+  simpl in *.
+  apply proj1_sig_eq in Heqpf. simpl in Heqpf. rewrite -Heqpf.
+  apply proj1_sig_eq in Heqd0. rewrite Heqd0.
+  apply proj1_sig_eq in Heqd. simpl in Heqd. rewrite -Heqd.
+  f_equal. f_equal.
+  { apply UIP_dec; apply bool_eqdec. }
+  { apply UIP_dec. apply bool_eqdec. }
+Qed.
+
+Lemma cast_proof_ml_goal_indifferent
+      Σ P Γ hyps goal goal' (e : goal = goal') (i : ProofInfo)
+      (pf : @mkMLGoal Σ Γ hyps goal i) wf1 wf2 wf3 wf4:
+  indifferent_to_cast P ->
+  P _ _ (proj1_sig (@cast_proof_ml_goal Σ Γ hyps goal goal' e i pf wf1 wf2)) = P _ _ (proj1_sig (pf wf3 wf4)).
+Proof.
+  intros Hp. simpl. unfold cast_proof_ml_goal.
+  unfold proj1_sig. unfold cast_proof'. destruct pf as [pf' Hpf'] eqn:Heqpf.
+  rewrite Hp.
+  apply f_equal. f_equal.
+  apply proj1_sig_eq in Heqpf. simpl in Heqpf. rewrite -Heqpf. clear Heqpf. simpl.
+  case_match. simpl in *.
+  apply proj1_sig_eq in Heqd. simpl in Heqd. rewrite -Heqd.
+  f_equal. f_equal.
+  { apply UIP_dec; apply bool_eqdec. }
+  { apply UIP_dec. apply bool_eqdec. }
+Qed.
+
+Lemma MLGoal_intro {Σ : Signature} (Γ : Theory) (l : list Pattern) (x g : Pattern)
+  (i : ProofInfo) :
+  @mkMLGoal Σ Γ (l ++ [x]) g i ->
+  @mkMLGoal Σ Γ l (x ---> g) i.
+Proof.
+  intros H.
+  unfold of_MLGoal in H. simpl in H.
+  unfold of_MLGoal. simpl. intros wfxig wfl.
+
+  feed specialize H.
+  { abstract (apply well_formed_imp_proj2 in wfxig; exact wfxig). }
+  { abstract (unfold Pattern.wf; unfold Pattern.wf in wfl; rewrite map_app foldr_app; simpl;
+              apply well_formed_imp_proj1 in wfxig; rewrite wfxig; simpl; exact wfl).
+  }
+  unshelve (eapply (cast_proof' _ H)).
+  { rewrite foldr_app. reflexivity. }
+Defined.
+
+Ltac simplLocalContext :=
+  match goal with
+    | [ |- @of_MLGoal ?Sgm (@mkMLGoal ?Sgm ?Ctx ?l ?g ?i) ]
+      => eapply cast_proof_ml_hyps;[(rewrite {1}[l]/app; reflexivity)|]
+  end.
+
+#[global]
+ Ltac mlIntro := apply MLGoal_intro; simplLocalContext.
+
+
+Local Example ex_toMLGoal {Σ : Signature} Γ (p : Pattern) :
+well_formed p ->
+Γ ⊢i p ---> p using BasicReasoning.
+Proof.
+intros wfp.
+toMLGoal.
+{ wf_auto2. }
+Set Printing All.
+match goal with
+| [ |- of_MLGoal (@mkMLGoal Σ Γ [] (p ---> p) BasicReasoning) ] => idtac
+| _ => fail
+end.
+fromMLGoal.
+Abort.
+
+
+Local Example ex_mlIntro {Σ : Signature} Γ a (i : ProofInfo) :
+well_formed a ->
+Γ ⊢i a ---> a using i.
+Proof.
+intros wfa.
+toMLGoal.
+{ wf_auto2. }
+mlIntro.
+match goal with
+| [ |- of_MLGoal (@mkMLGoal Σ Γ [a] a i) ] => idtac
+| _ => fail
+end.
+Abort.
+
+Lemma MLGoal_revert {Σ : Signature} (Γ : Theory) (l : list Pattern) (x g : Pattern) i :
+@mkMLGoal Σ Γ l (x ---> g) i ->
+@mkMLGoal Σ Γ (l ++ [x]) g i.
+Proof.
+intros H.
+unfold of_MLGoal in H. simpl in H.
+unfold of_MLGoal. simpl. intros wfxig wfl.
+
+feed specialize H.
+{
+  abstract (
+      apply wfapp_proj_2 in wfl;
+      unfold Pattern.wf in wfl;
+      simpl in wfl;
+      rewrite andbT in wfl;
+      wf_auto2
+    ).
+}
+{
+  abstract (apply wfapp_proj_1 in wfl; exact wfl).
+}
+
+eapply cast_proof'.
+{ rewrite foldr_app. simpl. reflexivity. }
+exact H.
+Defined.
+
+#[global]
+Ltac mlRevert :=
+match goal with
+| |- @of_MLGoal ?Sgm (@mkMLGoal ?Sgm ?Ctx ?l ?g ?i)
+=> eapply cast_proof_ml_hyps;
+   [(rewrite -[l](take_drop (length l - 1)); rewrite [take _ _]/=; rewrite [drop _ _]/=; reflexivity)|];
+   apply MLGoal_revert
+end.
+
+
+
+
+Lemma pile_evs_subseteq {Σ : Signature} evs1 evs2 svs kt fp:
+  evs1 ⊆ evs2 ->
+  ProofInfoLe
+    ((ExGen := evs1, SVSubst := svs, KT := kt, FP := fp))
+    ((ExGen := evs2, SVSubst := svs, KT := kt, FP := fp)).
+Proof.
+  intros Hsub.
+  constructor.
+  intros Γ ϕ pf Hpf.
+  destruct Hpf as [Hpf2 Hpf3 Hpf4 Hpf5].
+  constructor; simpl in *.
+  { clear -Hsub Hpf2. set_solver. }
+  { exact Hpf3. }
+  { exact Hpf4. }
+  { apply Hpf5. }
+Qed.
+
+Lemma pile_svs_subseteq {Σ : Signature} evs svs1 svs2 kt fp:
+  svs1 ⊆ svs2 ->
+  ProofInfoLe
+    ( (ExGen := evs, SVSubst := svs1, KT := kt, FP := fp))
+    ( (ExGen := evs, SVSubst := svs2, KT := kt, FP := fp)).
+Proof.
+  intros Hsub.
+  constructor.
+  intros Γ ϕ pf Hpf.
+  destruct Hpf as [Hpf2 Hpf3 Hpf4 Hpf5].
+  constructor; simpl in *.
+  { exact Hpf2. }
+  { clear -Hsub Hpf3. set_solver. }
+  { exact Hpf4. }
+  { exact Hpf5. }
+Qed.
+
+Lemma pile_kt_impl {Σ : Signature} evs svs kt1 kt2 fp:
+  kt1 ==> kt2 ->
+  ProofInfoLe
+    ((ExGen := evs, SVSubst := svs, KT := kt1, FP := fp))
+    ((ExGen := evs, SVSubst := svs, KT := kt2, FP := fp)).
+Proof.
+  intros Hsub.
+  constructor.
+  intros Γ ϕ pf Hpf.
+  destruct Hpf as [Hpf2 Hpf3 Hpf4 Hpf5].
+  constructor; simpl in *.
+  { exact Hpf2. }
+  { exact Hpf3. }
+  { unfold implb in *.  destruct (uses_kt pf),kt1; simpl in *; try reflexivity.
+    { exact Hsub. }
+    { inversion Hpf4. }
+  }
+  { apply Hpf5. }
+Qed.
+
+Lemma pile_fp_subseteq  {Σ : Signature} evs svs kt fp1 fp2:
+  fp1 ⊆ fp2 ->
+  ProofInfoLe
+    ((ExGen := evs, SVSubst := svs, KT := kt, FP := fp1))
+    ((ExGen := evs, SVSubst := svs, KT := kt, FP := fp2)).
+Proof.
+  intros Hsub.
+  constructor.
+  intros Γ ϕ pf Hpf.
+  destruct Hpf as [Hpf2 Hpf3 Hpf4 Hfp5].
+  constructor; simpl in *.
+  { exact Hpf2. }
+  { exact Hpf3. }
+  { exact Hpf4. }
+  { set_solver. }
+Qed.
