matching-logic/src/ProofMode_propositional.v
@@ -1,0 +1,3881 @@
+From Coq Require Import ssreflect ssrfun ssrbool.
+Set Implicit Arguments.
+Unset Strict Implicit.
+Unset Printing Implicit Defensive.
+
+From Ltac2 Require Import Ltac2.
+
+From Coq Require Import Ensembles Bool.
+From Coq.Logic Require Import FunctionalExtensionality Eqdep_dec.
+From Equations Require Import Equations.
+
+Require Import Coq.Program.Tactics.
+
+From MatchingLogic Require Import
+    Syntax
+    DerivedOperators_Syntax
+    ProofSystem
+    IndexManipulation
+    wftactics
+    ProofMode_base
+.
+
+From stdpp Require Import list tactics fin_sets coGset gmap sets.
+
+From MatchingLogic.Utils Require Import stdpp_ext.
+
+Import extralibrary.
+
+Import
+  MatchingLogic.Syntax.Notations
+  MatchingLogic.DerivedOperators_Syntax.Notations
+  MatchingLogic.ProofSystem.Notations
+.
+
+Set Default Proof Mode "Classic".
+
+Open Scope ml_scope.
+
+Lemma P1 {Σ : Signature} (Γ : Theory) (ϕ ψ : Pattern) :
+well_formed ϕ ->
+well_formed ψ ->
+Γ ⊢i ϕ ---> ψ ---> ϕ 
+using BasicReasoning.
+Proof.
+intros wfϕ wfψ.
+unshelve (eexists).
+{ apply ProofSystem.P1. exact wfϕ. exact wfψ. }
+{ abstract(solve_pim_simple). }
+Defined.
+
+Lemma P2 {Σ : Signature} (Γ : Theory) (ϕ ψ ξ : Pattern) :
+well_formed ϕ ->
+well_formed ψ ->
+well_formed ξ ->
+Γ ⊢i (ϕ ---> ψ ---> ξ) ---> (ϕ ---> ψ) ---> (ϕ ---> ξ)
+using BasicReasoning.
+Proof.
+intros wfϕ wfψ wfξ.
+unshelve (eexists).
+{ apply ProofSystem.P2. exact wfϕ. exact wfψ. exact wfξ. }
+{ abstract (solve_pim_simple). }
+Defined.
+
+Lemma P3 {Σ : Signature} (Γ : Theory) (ϕ : Pattern) :
+well_formed ϕ ->
+Γ ⊢i (((ϕ ---> ⊥) ---> ⊥) ---> ϕ)
+using BasicReasoning.
+Proof.
+intros wfϕ.
+unshelve (eexists).
+{ apply ProofSystem.P3. exact wfϕ. }
+{ abstract ( solve_pim_simple ). }
+Defined.
+
+Lemma MP {Σ : Signature} (Γ : Theory) (ϕ₁ ϕ₂ : Pattern) (i : ProofInfo) :
+Γ ⊢i ϕ₁ using i ->
+Γ ⊢i (ϕ₁ ---> ϕ₂) using i ->
+Γ ⊢i ϕ₂ using i.
+Proof.
+intros H1 H2.
+unshelve (eexists).
+{
+  eapply (ProofSystem.Modus_ponens _ _ _).
+  { apply H1. }
+  { apply H2. }
+}
+{
+  abstract(
+    simpl;
+    destruct H1 as [pf1 Hpf1];
+    destruct H2 as [pf2 Hpf2];
+    destruct Hpf1,Hpf2;
+    constructor; simpl;
+    [set_solver|set_solver|(destruct (uses_kt pf1),(uses_kt pf2); simpl in *; congruence)|set_solver]
+  ).
+}
+Defined.
+
+Lemma hypothesis {Σ : Signature} (Γ : Theory) (axiom : Pattern) :
+well_formed axiom ->
+(axiom ∈ Γ) ->
+Γ ⊢i axiom
+using BasicReasoning.
+Proof.
+intros Hwf Hin.
+unshelve (eexists).
+{
+  apply ProofSystem.hypothesis. apply Hwf. apply Hin.
+}
+{
+  abstract (
+    constructor; simpl;
+    [( set_solver )
+    |( set_solver )
+    |( reflexivity )
+    |( set_solver )
+    ]
+  ).
+}
+Defined.
+
+Arguments P1 {Σ} _ (_%ml) (_%ml) _ _ .
+Arguments P2 {Σ} _ (_%ml) (_%ml) (_%ml) _ _ _.
+Arguments P3 {Σ} _ (_%ml) _.
+
+  Lemma A_impl_A {Σ : Signature} (Γ : Theory) (A : Pattern)  :
+    (well_formed A) ->
+    Γ ⊢i (A ---> A)
+    using BasicReasoning.
+  Proof. 
+    intros WFA.
+    pose (_1 := P2 Γ A (A ---> A) A ltac:(wf_auto2) ltac:(wf_auto2) ltac:(wf_auto2)).
+    pose (_2 := P1 Γ A (A ---> A) ltac:(wf_auto2) ltac:(wf_auto2)).
+    pose (_3 := MP _2 _1).
+    pose (_4 := P1 Γ A A ltac:(wf_auto2) ltac:(wf_auto2)).
+    pose (_5 := MP _4 _3).
+    exact _5.
+  Defined.
+
+  Lemma P4m  {Σ : Signature}(Γ : Theory) (A B : Pattern) :
+    well_formed A ->
+    well_formed B ->
+    Γ ⊢i ((A ---> B) ---> ((A ---> !B) ---> !A))
+    using BasicReasoning.
+  Proof.
+    intros WFA WFB.
+    pose (H1 := P2 Γ A B Bot ltac:(wf_auto2) ltac:(wf_auto2) ltac:(wf_auto2)).
+    pose (H2 := (P2 Γ (A ---> B ---> Bot) (A ---> B) (A ---> Bot) ltac:(wf_auto2) ltac:(wf_auto2) ltac:(wf_auto2))).
+    pose (H3 := MP H1 H2).
+    pose (H4 := (P1 Γ (((A ---> B ---> Bot) ---> A ---> B) ---> (A ---> B ---> Bot) ---> A ---> Bot)
+      (A ---> B) ltac:(wf_auto2) ltac:(wf_auto2))).
+    pose (H5 := MP  H3 H4).
+    pose (H6 := (P2 Γ (A ---> B) ((A ---> B ---> Bot) ---> A ---> B) ((A ---> B ---> Bot) ---> A ---> Bot)
+      ltac:(wf_auto2) ltac:(wf_auto2) ltac:(wf_auto2))).
+    pose (H7 := MP H5 H6).
+    pose (H8 := (P1 Γ (A ---> B) (A ---> B ---> Bot) ltac:(wf_auto2) ltac:(wf_auto2))).
+    pose (H9 := MP H8 H7).
+    exact H9.
+  Defined.
+
+  Lemma P4i {Σ : Signature} (Γ : Theory) (A : Pattern) :
+    well_formed A ->
+    Γ ⊢i ((A ---> !A) ---> !A)
+    using BasicReasoning.
+  Proof.
+    intros WFA.
+    eapply MP.
+    { apply (@A_impl_A _ _ A WFA). }
+    { apply (@P4m _ _ A A WFA WFA). }
+  Defined.
+
+  Lemma reorder {Σ : Signature} (Γ : Theory) (A B C : Pattern) :
+    well_formed A ->
+    well_formed B ->
+    well_formed C ->
+    Γ ⊢i ((A ---> B ---> C) ---> ( B ---> A ---> C))
+    using BasicReasoning.
+  Proof.
+    intros WFA WFB WFC.
+   
+    pose (t1 := (MP
+                    (P1 Γ ((A ---> B) ---> A ---> C) B ltac:(wf_auto2) ltac:(wf_auto2))
+                    (P1 Γ (((A ---> B) ---> A ---> C) ---> B ---> (A ---> B) ---> A ---> C) (A ---> B ---> C) ltac:(wf_auto2) ltac:(wf_auto2)))).
+  
+    pose(ABC := (A ---> B ---> C)).
+    
+    eapply MP.
+    - eapply MP.
+      + apply(P1 _ B A ltac:(wf_auto2) ltac:(wf_auto2)).
+      + apply(P1 _ (B ---> A ---> B) (A ---> B ---> C) ltac:(wf_auto2) ltac:(wf_auto2)).
+    - eapply MP.
+      + eapply MP.
+        * eapply MP.
+          -- eapply MP.
+             ++ apply (@A_impl_A _ _ ABC ltac:(wf_auto2)).
+             ++ eapply MP.
+                ** eapply MP.
+                   --- apply(P2 _ A B C ltac:(wf_auto2) ltac:(wf_auto2) ltac:(wf_auto2)).
+                   --- unshelve (eapply(P1 _ _ (A ---> B ---> C) _ _)); wf_auto2.
+                ** apply P2; wf_auto2.
+          -- eapply MP.
+             ++ apply t1.
+             ++ apply(P2 _ ABC ((A ---> B) ---> (A ---> C)) (B ---> (A ---> B) ---> (A ---> C)) ltac:(wf_auto2) ltac:(wf_auto2) ltac:(wf_auto2)).
+        * eapply MP.
+          -- eapply MP.
+             ++ apply(P2 _ B (A ---> B) (A ---> C) ltac:(wf_auto2) ltac:(wf_auto2) ltac:(wf_auto2)).
+             ++ apply(P1 _ _ ABC); wf_auto2.
+          -- apply P2; wf_auto2.
+      + apply P2; wf_auto2.
+  Defined.
+
+
+  Lemma reorder_meta {Σ : Signature} (Γ : Theory) (A B C : Pattern) (i : ProofInfo) :
+    well_formed A ->
+    well_formed B ->
+    well_formed C ->  
+    Γ ⊢i (A ---> B ---> C) using i ->
+    Γ ⊢i (B ---> A ---> C) using i.
+  Proof.
+    intros H H0 H1 H2.
+    eapply MP. apply H2.
+    apply useBasicReasoning.
+    apply reorder; wf_auto2.
+  Defined.
+
+  Lemma syllogism {Σ : Signature} (Γ : Theory) (A B C : Pattern) :
+    well_formed A ->
+    well_formed B ->
+    well_formed C ->
+    Γ ⊢i ((A ---> B) ---> (B ---> C) ---> (A ---> C))
+    using BasicReasoning.
+  Proof.
+    intros WFA WFB WFC.
+    apply reorder_meta;[wf_auto2|wf_auto2|wf_auto2|].
+    eapply MP.
+    - apply(P1 _ (B ---> C) A); wf_auto2.
+    - eapply MP.
+      + eapply MP.
+        * apply (P2 _ A B C); wf_auto2.
+        * apply (P1 _ ((A ---> B ---> C) ---> (A ---> B) ---> A ---> C) (B ---> C)); wf_auto2.
+      + apply P2; wf_auto2.
+  Defined.
+  
+  Lemma syllogism_meta {Σ : Signature} (Γ : Theory) (A B C : Pattern) (i : ProofInfo) :
+    well_formed A ->
+    well_formed B ->
+    well_formed C ->
+    Γ ⊢i (A ---> B) using i ->
+    Γ ⊢i (B ---> C) using i ->
+    Γ ⊢i (A ---> C) using i.
+  Proof.
+    intros H H0 H1 H2 H3.
+    eapply MP.
+    - exact H2.
+    - eapply MP.
+      + exact H3.
+      + apply reorder_meta;[wf_auto2|wf_auto2|wf_auto2|].
+        apply useBasicReasoning.
+        apply syllogism; wf_auto2.
+  Defined.
+  
+  Lemma modus_ponens {Σ : Signature} (Γ : Theory) (A B : Pattern) :
+    well_formed A ->
+    well_formed B ->
+    Γ ⊢i (A ---> (A ---> B) ---> B)
+    using BasicReasoning.
+  Proof.
+    intros WFA WFB.
+    eapply MP.
+    - apply (P1 _ A (A ---> B) ltac:(wf_auto2) ltac:(wf_auto2)).
+    - eapply MP.
+      + eapply MP.
+        * apply (@A_impl_A _ _ (A ---> B) ltac:(wf_auto2)).
+        * eapply (P2 _ (A ---> B) A B ltac:(wf_auto2) ltac:(wf_auto2) ltac:(wf_auto2)).
+      + apply reorder_meta;[wf_auto2|wf_auto2|wf_auto2|].
+        apply syllogism; wf_auto2.
+  Defined.
+
+  Lemma not_not_intro {Σ : Signature} (Γ : Theory) (A : Pattern) :
+    well_formed A ->
+    Γ ⊢i (A ---> !(!A))
+    using BasicReasoning.
+  Proof.
+    intros WFA.
+    apply modus_ponens; wf_auto2.
+  Defined.
+
+  Lemma P4 {Σ : Signature} (Γ : Theory) (A B : Pattern)  :
+    well_formed A ->
+    well_formed B -> 
+    Γ ⊢i (((! A) ---> (! B)) ---> (B ---> A))
+    using BasicReasoning.
+  Proof.
+    intros WFA WFB.
+    pose proof (m := P3 Γ A ltac:(wf_auto2)).
+    pose proof (m0 := P1 Γ (((A ---> Bot) ---> Bot) ---> A) B ltac:(wf_auto2) ltac:(wf_auto2)).
+    pose proof (m1 := P2 Γ B ((A ---> Bot) ---> Bot) A ltac:(wf_auto2) ltac:(wf_auto2) ltac:(wf_auto2)).
+    pose proof (m2 := MP m m0).
+    pose proof (m3 := MP m2 m1).
+    pose proof (m4 := P1 Γ ((B ---> (A ---> Bot) ---> Bot) ---> B ---> A) ((A ---> Bot) ---> (B ---> Bot)) ltac:(wf_auto2) ltac:(wf_auto2) ).
+    pose proof (m5 := MP m3 m4).
+    pose proof (m6 := P2 Γ ((A ---> Bot) ---> (B ---> Bot)) (B ---> (A ---> Bot) ---> Bot) (B ---> A) ltac:(wf_auto2) ltac:(wf_auto2) ltac:(wf_auto2)).
+    pose proof (m7 := MP m5 m6).
+    pose proof (m8 := @reorder _ Γ (A ---> Bot) (B) Bot ltac:(wf_auto2) ltac:(wf_auto2) ltac:(wf_auto2)).
+    apply (MP m8 m7).
+  Defined.
+
+  Lemma conj_intro {Σ : Signature} (Γ : Theory) (A B : Pattern) :
+    well_formed A ->
+    well_formed B ->
+    Γ ⊢i (A ---> B ---> (A and B))
+    using BasicReasoning.
+  Proof.
+    intros WFA WFB.
+    pose proof (tB := (@A_impl_A _ Γ B ltac:(wf_auto2))).
+    epose proof (t1 := MP (P2 _ (!(!A) ---> !B) A Bot ltac:(wf_auto2) ltac:(wf_auto2) ltac:(wf_auto2)) (P1 _ _ B _ _)).
+    epose proof (t2 := MP (reorder_meta _ _ _ (@P4 _ _ (!A) B ltac:(wf_auto2) ltac:(wf_auto2))) (P1 _ _ B _ _)).
+    epose proof (t3'' := MP (P1 _ A (!(!A) ---> !B) _ _) (P1 _ _ B _ _)).
+    epose proof (t4 := MP tB (MP t2 (P2 _ B B _ _ _ _))).
+    epose proof (t5'' := 
+            MP t4
+                         (MP t1
+                                       (P2 _ B ((!(!A) ---> !B) ---> !A)
+                                           (((!(!A) ---> !B) ---> A) ---> !(!(!A) ---> !B)) _ _ _))).
+    
+    epose proof (tA := (P1 Γ A B) _ _).
+    epose proof (tB' := MP tB
+                              (P1 _ (B ---> B) A _ _)).
+    epose proof (t3' := MP t3''
+                              (P2 _ B A ((!(!A) ---> !B) ---> A) _ _ _)).
+    epose proof (t3 := MP t3'
+                             (P1 _ ((B ---> A) ---> B ---> (! (! A) ---> ! B) ---> A) A _ _)).
+    epose proof (t5' := MP t5''
+                              (P2 _ B ((!(!A) ---> !B) ---> A) (!(!(!A) ---> !B)) _ _ _)).
+    epose proof (t5 := MP t5' 
+                             (P1 _ ((B ---> (! (! A) ---> ! B) ---> A) ---> B ---> ! (! (! A) ---> ! B))
+                                 A _ _)).
+    epose proof (t6 := MP tA
+                             (MP t3
+                                           (P2 _ A (B ---> A) (B ---> (!(!A) ---> !B) ---> A) _ _ _))).
+    epose proof (t7 := MP t6 
+                             (MP t5 
+                                           (P2 _ A (B ---> (!(!A) ---> !B) ---> A) (B ---> !(!(!A) ---> !B)) _ _ _))).
+    apply t7.
+    Unshelve.
+    all: wf_auto2.
+  Defined.
+
+  Lemma conj_intro_meta {Σ : Signature} (Γ : Theory) (A B : Pattern) (i : ProofInfo) :
+    well_formed A ->
+    well_formed B ->
+    Γ ⊢i A using i ->
+    Γ ⊢i B using i ->
+    Γ ⊢i (A and B) using i.
+  Proof.
+    intros WFA WFB H H0.
+    eapply MP.
+    - exact H0.
+    - eapply MP.
+      + exact H.
+      + apply useBasicReasoning.
+        apply conj_intro; wf_auto2.
+  Defined.
+  
+  Lemma syllogism_4_meta {Σ : Signature} (Γ : Theory) (A B C D : Pattern) (i : ProofInfo) :
+    well_formed A ->
+    well_formed B ->
+    well_formed C ->
+    well_formed D ->
+    Γ ⊢i (A ---> B ---> C) using i ->
+    Γ ⊢i (C ---> D) using i ->
+    Γ ⊢i (A ---> B ---> D) using i.
+  Proof.
+    intros WFA WFB WFC WFD H H0.
+    eapply MP.
+    - exact H.
+    - eapply MP.
+      + eapply MP.
+        * eapply MP.
+          -- eapply MP.
+             ++ exact H0.
+             ++ apply useBasicReasoning. 
+                eapply (P1 _ (C ---> D) B _ _).
+          -- apply useBasicReasoning.  
+              eapply (P2 _ B C D _ _ _).
+        * apply useBasicReasoning. 
+          eapply (P1 _ ((B ---> C) ---> B ---> D) A _ _).
+      + apply useBasicReasoning. 
+        eapply (P2 _ A (B ---> C) (B ---> D) _ _ _).
+        Unshelve.
+        all: wf_auto2.
+  Defined.
+
+  Lemma bot_elim {Σ : Signature} (Γ : Theory) (A : Pattern) :
+    well_formed A ->
+    Γ ⊢i (Bot ---> A)
+    using BasicReasoning.
+  Proof.
+    intros WFA.
+    eapply MP.
+    - eapply MP.
+      + eapply MP.
+        * eapply MP.
+          -- eapply (P1 _ Bot Bot _ _).
+          -- eapply (P2 _ Bot Bot Bot _ _ _).
+        * eapply (@P4 _ _ Bot Bot _ _).
+      + eapply (P1 _ (Bot ---> Bot) (A ---> Bot) _ _).
+    - eapply (@P4 _ _ A Bot _ _).
+      Unshelve.
+      all: wf_auto2.
+  Defined.
+
+  Lemma modus_ponens' {Σ : Signature} (Γ : Theory) (A B : Pattern) :
+    well_formed A ->
+    well_formed B ->
+    Γ ⊢i (A ---> (!B ---> !A) ---> B)
+    using BasicReasoning.
+  Proof.
+    intros WFA WFB.
+    apply reorder_meta;[wf_auto2|wf_auto2|wf_auto2|].
+    apply P4; wf_auto2.
+  Defined.
+
+  Lemma disj_right_intro {Σ : Signature} (Γ : Theory) (A B : Pattern) :
+    well_formed A ->
+    well_formed B ->
+    Γ ⊢i (B ---> (A or B))
+    using BasicReasoning.
+  Proof.
+    intros WFA WFB.
+    apply useBasicReasoning.
+    apply P1; wf_auto2.
+  Defined.
+  
+  Lemma disj_left_intro {Σ : Signature} (Γ : Theory) (A B : Pattern) :
+    well_formed A ->
+    well_formed B ->
+    Γ ⊢i (A ---> (A or B))
+    using BasicReasoning.
+  Proof.
+    intros WFA WFB.
+    eapply syllogism_4_meta.
+    5: { apply modus_ponens; wf_auto2. }
+    5: { apply bot_elim; wf_auto2. }
+    all: wf_auto2.
+  Defined.
+
+  Lemma disj_right_intro_meta {Σ : Signature} (Γ : Theory) (A B : Pattern) (i : ProofInfo) :
+    well_formed A ->
+    well_formed B ->
+    Γ ⊢i B using i ->
+    Γ ⊢i (A or B) using i.
+  Proof.
+    intros HwfA HwfB HB.
+    eapply MP.
+    { exact HB. }
+    {
+      apply useBasicReasoning.
+      apply disj_right_intro; wf_auto2.
+    }
+  Defined.
+
+  Lemma disj_left_intro_meta {Σ : Signature} (Γ : Theory) (A B : Pattern) (i : ProofInfo) :
+    well_formed A ->
+    well_formed B ->
+    Γ ⊢i A using i ->
+    Γ ⊢i (A or B) using i.
+  Proof.
+    intros HwfA HwfB HA.
+    eapply MP.
+    { exact HA. }
+    apply useBasicReasoning.
+    apply disj_left_intro; assumption.
+  Defined.
+
+  Lemma not_not_elim {Σ : Signature} (Γ : Theory) (A : Pattern) :
+    well_formed A ->
+    Γ ⊢i (!(!A) ---> A)
+    using BasicReasoning.
+  Proof.
+    intros WFA.
+    apply P3. exact WFA.
+  Defined.
+
+  Lemma not_not_elim_meta {Σ : Signature} Γ A (i : ProofInfo) :
+    well_formed A ->
+    Γ ⊢i (! ! A) using i ->
+    Γ ⊢i A using i.
+  Proof.
+    intros wfA nnA.
+    eapply MP.
+    { apply nnA. }
+    { apply useBasicReasoning. apply not_not_elim. exact wfA. }
+  Defined.
+
+  Lemma double_neg_elim {Σ : Signature} (Γ : Theory) (A B : Pattern) :
+    well_formed A ->
+    well_formed B ->
+    Γ ⊢i (((!(!A)) ---> (!(!B))) ---> (A ---> B))
+    using BasicReasoning.
+  Proof.
+    intros WFA WFB.
+    eapply syllogism_meta.
+    5: apply P4.
+    4: apply P4.
+    all: wf_auto2.
+  Defined.
+
+  Lemma double_neg_elim_meta {Σ : Signature} (Γ : Theory) (A B : Pattern) (i : ProofInfo) :
+    well_formed A ->
+    well_formed B -> 
+    Γ ⊢i ((!(!A)) ---> (!(!B))) using i ->
+    Γ ⊢i (A ---> B) using i.
+  Proof.
+    intros WFA WFB H.
+    eapply MP.
+    - exact H.
+    - apply useBasicReasoning.
+      apply double_neg_elim; wf_auto2.
+  Defined.
+
+  Lemma not_not_impl_intro {Σ : Signature} (Γ : Theory) (A B : Pattern) :
+    well_formed A ->
+    well_formed B ->
+    Γ ⊢i ((A ---> B) ---> ((! ! A) ---> (! ! B)))
+    using BasicReasoning.
+  Proof.
+    intros WFA WFB.
+    
+    epose (S1 := @syllogism _ Γ (! ! A) A B _ _ _).
+    
+    epose (MP1 := MP (@not_not_elim _ _ A _) S1).
+    
+    epose(NNB := @not_not_intro _ Γ B _).
+
+    epose(P1 := (P1 Γ (B ---> ! (! B)) (! ! A) _ _)).
+    
+    epose(MP2 := MP NNB P1).
+    
+    epose(P2' := (P2 Γ (! ! A) B (! !B) _ _ _)).
+    
+    epose(MP3 := MP MP2 P2').
+    
+    eapply @syllogism_meta with (B := (! (! A) ---> B)).
+    - shelve.
+    - shelve.
+    - shelve.
+    - assumption.
+    - assumption.
+      Unshelve.
+      all: wf_auto2.
+  Defined.
+
+  Lemma contraposition {Σ : Signature} (Γ : Theory) (A B : Pattern) : 
+    well_formed A ->
+    well_formed B -> 
+    Γ ⊢i ((A ---> B) ---> ((! B) ---> (! A)))
+    using BasicReasoning.
+  Proof.
+    intros WFA WFB.
+    epose proof (@P4 _ Γ (! A) (! B) _ _) as m.
+    apply syllogism_meta with (B := (! (! A) ---> ! (! B))).
+    - shelve.
+    - shelve.
+    - shelve.
+    - apply @not_not_impl_intro; wf_auto2.
+    - exact m. (* apply (P4 _ _ _). shelve. shelve. *)
+      Unshelve.
+      all: wf_auto2.
+  Defined.
+
+  Lemma or_comm_meta {Σ : Signature} (Γ : Theory) (A B : Pattern) (i : ProofInfo):
+    well_formed A ->
+    well_formed B ->
+    Γ ⊢i (A or B) using i ->
+    Γ ⊢i (B or A) using i.
+  Proof.
+    intros WFA WFB H. unfold patt_or in *.    
+    epose proof (P4 := (@P4 _ Γ A (!B) _ _)).
+    epose proof (NNI := @not_not_intro  _ Γ B _).
+    apply (useBasicReasoning i) in P4.
+    apply (useBasicReasoning i) in NNI.
+    epose proof (SI := @syllogism_meta _ Γ _ _ _ _ _ _ _ H NNI).
+    eapply MP.
+    - exact SI.
+    - exact P4.
+      Unshelve.
+      all: wf_auto2.
+  Defined.
+
+  Lemma A_implies_not_not_A_alt {Σ : Signature} (Γ : Theory) (A : Pattern) (i : ProofInfo) :
+    well_formed A ->
+    Γ ⊢i A using i ->
+    Γ ⊢i (!( !A )) using i.
+  Proof.
+    intros WFA H. unfold patt_not.
+    eapply MP.
+    { apply H. }
+    {
+      apply useBasicReasoning.
+      apply not_not_intro.
+      exact WFA.
+    }
+  Defined.
+
+  Lemma P5i {Σ : Signature} (Γ : Theory) (A B : Pattern) :
+    well_formed A ->
+    well_formed B ->
+    Γ ⊢i (! A ---> (A ---> B))
+    using BasicReasoning.
+  Proof.
+    intros WFA WFB.
+    eapply syllogism_meta.
+    5: apply P4.
+    4: apply P1.
+    all: wf_auto2.
+  Defined.
+
+  Lemma false_implies_everything {Σ : Signature} (Γ : Theory) (phi : Pattern) :
+    well_formed phi ->
+    Γ ⊢i (Bot ---> phi) using BasicReasoning.
+  Proof.
+    apply bot_elim.
+  Defined.
+
+  Lemma A_implies_not_not_A_alt_Γ {Σ : Signature} (Γ : Theory) (A : Pattern) (i : ProofInfo) :
+    well_formed A ->
+    Γ ⊢i A using i ->
+    Γ ⊢i (!( !A )) using i.
+  Proof.
+    intros WFA H. unfold patt_not.
+    eapply MP.
+    { apply H. }
+    { apply useBasicReasoning. apply not_not_intro. exact WFA. }
+  Defined.
+
+
+  Lemma exclusion {Σ : Signature} (G : Theory) (A : Pattern) (i : ProofInfo) :
+    well_formed A ->
+    G ⊢i A using i ->
+    G ⊢i (A ---> Bot) using i ->
+    G ⊢i Bot using i.
+  Proof.
+    intros WFA H H0.
+    eapply MP.
+    apply H.
+    apply H0.
+  Defined.
+
+  Lemma modus_tollens {Σ : Signature} Γ A B (i : ProofInfo) :
+    Γ ⊢i (A ---> B) using i ->
+    Γ ⊢i (!B ---> !A) using i.
+  Proof.
+    intros H.
+    pose proof (wf := proved_impl_wf _ _ (proj1_sig H)).
+    assert (wfA : well_formed A) by wf_auto2.
+    assert (wfB : well_formed B) by wf_auto2.
+
+    eapply MP.
+    2: { apply useBasicReasoning. apply contraposition; wf_auto2. }
+    apply H.
+  Defined.
+  
+  Lemma A_impl_not_not_B {Σ : Signature} Γ A B :
+    well_formed A ->
+    well_formed B ->
+    Γ ⊢i ((A ---> ! !B) ---> (A ---> B))
+    using BasicReasoning.
+  Proof.
+    intros WFA WFB.
+
+    assert (H0 : Γ ⊢i (! !B ---> B) using BasicReasoning).
+    {
+      apply not_not_elim. wf_auto2.
+    }
+
+    assert (H1 : Γ ⊢i ((A ---> ! !B) ---> (! !B ---> B) ---> (A ---> B)) using BasicReasoning).
+    {
+      apply syllogism; wf_auto2.
+    }
+
+    eapply MP.
+    2: { 
+      apply reorder_meta.
+      4: apply H1.
+      all: wf_auto2.
+    }
+    apply H0.
+  Defined.
+
+  Lemma prf_weaken_conclusion {Σ : Signature} Γ A B B' :
+    well_formed A ->
+    well_formed B ->
+    well_formed B' ->
+    Γ ⊢i ((B ---> B') ---> ((A ---> B) ---> (A ---> B')))
+    using BasicReasoning.
+  Proof.
+    intros wfA wfB wfB'.
+    apply reorder_meta;[wf_auto2|wf_auto2|wf_auto2|].
+    apply syllogism; wf_auto2.
+  Defined.
+
+  Lemma prf_weaken_conclusion_meta {Σ : Signature} Γ A B B' (i : ProofInfo) :
+    well_formed A ->
+    well_formed B ->
+    well_formed B' ->
+    Γ ⊢i (B ---> B') using i ->
+    Γ ⊢i ((A ---> B) ---> (A ---> B')) using i.
+  Proof.
+    intros wfA wfB wfB' BimpB'.
+    assert (H1: Γ ⊢i ((A ---> B) ---> (B ---> B') ---> (A ---> B')) using i).
+    {
+      apply useBasicReasoning. apply syllogism; wf_auto2.
+    }
+    apply reorder_meta in H1;[|wf_auto2|wf_auto2|wf_auto2].
+    eapply MP. 2: apply H1. apply BimpB'.
+  Defined.
+
+  Lemma prf_weaken_conclusion_iter {Σ : Signature} Γ l g g'
+          (wfl : Pattern.wf l) (wfg : well_formed g) (wfg' : well_formed g') :
+    Γ ⊢i ((g ---> g') ---> (fold_right patt_imp g l ---> fold_right patt_imp g' l))
+    using BasicReasoning.
+  Proof.
+    induction l.
+    - apply A_impl_A. wf_auto2.
+    - pose proof (wfl' := wfl).
+      apply andb_prop in wfl.
+      fold (map well_formed) in wfl.
+      destruct wfl as [wfa wfl].
+      (* I do not know how to fold it, so I just assert & clear. *)
+      assert (wfl'' : Pattern.wf l) by apply wfl.
+      clear wfl.
+      specialize (IHl wfl'').
+      simpl in *.
+      eapply syllogism_meta.
+      5: eapply prf_weaken_conclusion.
+      4: apply IHl.
+      all: wf_auto2.
+  Defined.
+
+  Lemma prf_weaken_conclusion_iter_meta {Σ : Signature} Γ l g g' (i : ProofInfo):
+    Pattern.wf l ->
+    well_formed g ->
+    well_formed g' ->
+    Γ ⊢i (g ---> g') using i ->
+    Γ ⊢i ((fold_right patt_imp g l) ---> (fold_right patt_imp g' l)) using i.
+  Proof.
+    intros wfl wfg wfg' gimpg'.
+    eapply MP.
+    2: { apply useBasicReasoning. apply prf_weaken_conclusion_iter; wf_auto2. }
+    1: { apply gimpg'. }
+  Defined.
+
+  Lemma prf_weaken_conclusion_iter_meta_meta {Σ : Signature} Γ l g g' (i : ProofInfo):
+    Pattern.wf l ->
+    well_formed g ->
+    well_formed g' ->
+    Γ ⊢i (g ---> g') using i ->
+    Γ ⊢i (fold_right patt_imp g l) using i ->
+    Γ ⊢i (fold_right patt_imp g' l) using i.
+  Proof.
+    intros wfl wfg wfg' gimpg' H.
+    eapply MP.
+    { apply gimpg'. }
+    eapply MP.
+    { apply H. }
+    apply reorder_meta;[wf_auto2|wf_auto2|wf_auto2|].
+    apply useBasicReasoning.
+    apply prf_weaken_conclusion_iter.
+    all: wf_auto2.
+  Defined.
+
+  Lemma prf_weaken_conclusion_meta_meta {Σ : Signature} Γ A B B' (i : ProofInfo) :
+    well_formed A ->
+    well_formed B ->
+    well_formed B' ->
+    Γ ⊢i (B ---> B') using i ->
+    Γ ⊢i (A ---> B) using i ->
+    Γ ⊢i (A ---> B') using i.
+  Proof.
+    intros WFA WFB WFB' H H0.
+    eapply MP. 2: apply prf_weaken_conclusion_meta. 1: apply H0.
+    4: apply H. all: wf_auto2.
+  Defined.
+
+  Lemma prf_strenghten_premise {Σ : Signature} Γ A A' B :
+    well_formed A ->
+    well_formed A' ->
+    well_formed B ->
+    Γ ⊢i ((A' ---> A) ---> ((A ---> B) ---> (A' ---> B))) using BasicReasoning.
+  Proof.
+    intros wfA wfA' wfB.
+    apply syllogism; wf_auto2.
+  Defined.
+
+  Lemma prf_strenghten_premise_iter {Σ : Signature}  Γ l₁ l₂ h h' g :
+    Pattern.wf l₁ -> Pattern.wf l₂ ->
+    well_formed h ->
+    well_formed h' ->
+    well_formed g ->
+    Γ ⊢i (h' ---> h) --->
+        foldr patt_imp g (l₁ ++ h::l₂) --->
+        foldr patt_imp g (l₁ ++ h'::l₂)
+    using BasicReasoning.
+  Proof.
+    intros wfl₁ wfl₂ wfh wfh' wfg.
+    induction l₁.
+    - simpl. apply prf_strenghten_premise. all: wf_auto2.
+    - pose proof (wfal₁ := wfl₁).
+      remember (foldr patt_imp g (h::l₂)) as g1.
+      remember (foldr patt_imp g (h'::l₂)) as g2.
+      unfold Pattern.wf in wfl₁. simpl in wfl₁. apply andb_prop in wfl₁.
+      destruct wfl₁ as [wfa wfl₁].
+      specialize (IHl₁ wfl₁).
+      remember (foldr patt_imp g (l₁ ++ h::l₂)) as b.
+      remember (foldr patt_imp g (l₁ ++ h'::l₂)) as b'.
+
+      assert (prf: Γ ⊢i ((b ---> b') ---> ((a ---> b) ---> (a ---> b'))) using BasicReasoning).
+      { apply prf_weaken_conclusion; subst; wf_auto2. }
+
+      subst.
+      eapply syllogism_meta.
+      5: { apply prf. }
+      4: { apply IHl₁. }
+      all: wf_auto2.
+  Defined.
+
+  Lemma prf_strenghten_premise_meta {Σ : Signature} Γ A A' B (i : ProofInfo) :
+    well_formed A ->
+    well_formed A' ->
+    well_formed B ->
+    Γ ⊢i (A' ---> A) using i ->
+    Γ ⊢i ((A ---> B) ---> (A' ---> B)) using i.
+  Proof.
+    intros wfA wfA' wfB A'impA.
+    assert (H1: Γ ⊢i ((A' ---> A) ---> (A ---> B) ---> (A' ---> B)) using i).
+    {
+      apply useBasicReasoning. apply syllogism; wf_auto2.
+    }
+    eapply MP. 2: apply H1. apply A'impA.
+  Defined.
+
+  Lemma prf_strenghten_premise_meta_meta {Σ : Signature} Γ A A' B (i : ProofInfo) :
+    well_formed A ->
+    well_formed A' ->
+    well_formed B ->
+    Γ ⊢i (A' ---> A) using i ->
+    Γ ⊢i (A ---> B) using i ->
+    Γ ⊢i (A' ---> B) using i.
+  Proof.
+    intros wfA wfA' wfB A'impA AimpB.
+    eapply MP. 2: apply prf_strenghten_premise_meta. 1: apply AimpB.
+    4: apply A'impA. all: wf_auto2.
+  Defined.
+
+  Lemma prf_strenghten_premise_iter_meta {Σ : Signature} Γ l₁ l₂ h h' g (i : ProofInfo) :
+    Pattern.wf l₁ -> Pattern.wf l₂ ->
+    well_formed h ->
+    well_formed h' ->
+    well_formed g ->
+    Γ ⊢i (h' ---> h) using i ->
+    Γ ⊢i foldr patt_imp g (l₁ ++ h::l₂) --->
+         foldr patt_imp g (l₁ ++ h'::l₂)
+    using i.  
+  Proof.
+    intros WFl₁ WFl₂ WFh WFh' WFg H.
+    eapply MP.
+    2: { apply useBasicReasoning. apply prf_strenghten_premise_iter; wf_auto2. }
+    exact H.
+  Defined.
+
+  Lemma prf_strenghten_premise_iter_meta_meta {Σ : Signature} Γ l₁ l₂ h h' g (i : ProofInfo) :
+    Pattern.wf l₁ -> Pattern.wf l₂ ->
+    well_formed h ->
+    well_formed h' ->
+    well_formed g ->
+    Γ ⊢i (h' ---> h) using i ->
+    Γ ⊢i foldr patt_imp g (l₁ ++ h::l₂) using i ->
+    Γ ⊢i foldr patt_imp g (l₁ ++ h'::l₂) using i.  
+  Proof.
+    intros WFl₁ WFl₂ WFh WFh' WFg H H0.
+    eapply MP.
+    2: eapply prf_strenghten_premise_iter_meta.
+    7: eassumption. 1: assumption. all: wf_auto2.
+  Defined.
+
+
+  Local Example example_nested_const {Σ : Signature} Γ a b c:
+    well_formed a ->
+    well_formed b ->
+    well_formed c ->
+    (* like P2 but nested a bit *)
+    Γ ⊢i (a ---> (b ---> (c ---> a)))
+    using BasicReasoning.
+  Proof.
+    intros wfa wfb wfc.
+    assert (H1: Γ ⊢i ((c ---> a) ---> (b ---> (c ---> a))) using BasicReasoning).
+    {
+      apply P1; wf_auto2.
+    }
+    assert (H2: Γ ⊢i (a ---> (c ---> a)) using BasicReasoning).
+    { apply P1; wf_auto2. }
+
+    eapply (@syllogism_meta _ _ _ _ _ _ _ _ _ H2 H1).
+    Unshelve. all: wf_auto2.
+  Defined.
+
+  (* This will form a base for the tactic 'exact 0' *)
+  Lemma nested_const {Σ : Signature} Γ a l:
+    well_formed a ->
+    Pattern.wf l ->
+    Γ ⊢i (a ---> (fold_right patt_imp a l))
+    using BasicReasoning.
+  Proof.
+    intros wfa wfl.
+    induction l; simpl.
+    - apply A_impl_A. exact wfa.
+    - pose proof (wfa0l := wfl).
+      unfold Pattern.wf in wfl. simpl in wfl. apply andb_prop in wfl. destruct wfl as [wfa0 wfl].
+      specialize (IHl wfl).
+      assert (H1 : Γ ⊢i ((foldr patt_imp a l) ---> (a0 ---> (foldr patt_imp a l))) using BasicReasoning).
+      {
+        apply P1; wf_auto2.
+      }
+      eapply syllogism_meta.
+      5: apply H1. 4: assumption. all: wf_auto2.
+  Defined.
+
+  Lemma nested_const_middle {Σ : Signature} Γ a l₁ l₂:
+    well_formed a ->
+    Pattern.wf l₁ ->
+    Pattern.wf l₂ ->
+    Γ ⊢i (fold_right patt_imp a (l₁ ++ a :: l₂))
+    using BasicReasoning.
+  Proof.
+    intros wfa wfl₁ wfl₂.
+    induction l₁; simpl.
+    - apply nested_const; wf_auto2.
+    - pose proof (wfa0l₁ := wfl₁).
+      unfold Pattern.wf in wfl₁. simpl in wfl₁. apply andb_prop in wfl₁. destruct wfl₁ as [wfa0 wfl₁].
+      specialize (IHl₁ wfl₁). simpl in IHl₁.
+      eapply MP. 2: apply P1. 1: apply IHl₁. all: wf_auto2.
+  Defined.
+
+  Lemma prf_reorder_iter {Σ : Signature} Γ a b g l₁ l₂:
+    well_formed a ->
+    well_formed b ->
+    well_formed g ->
+    Pattern.wf l₁ ->
+    Pattern.wf l₂ ->
+    Γ ⊢i ((fold_right patt_imp g (l₁ ++ [a;b] ++ l₂)) --->
+         (fold_right patt_imp g (l₁ ++ [b;a] ++ l₂)))
+    using BasicReasoning.
+  Proof.
+    intros wfa wfb wfg wfl₁ wfl₂.
+    induction l₁; simpl in *.
+    - apply reorder; wf_auto2.
+    - pose proof (wfa0l₁ := wfl₁).
+      unfold Pattern.wf in wfl₁. apply andb_prop in wfl₁. destruct wfl₁ as [wfa0 wfl₁].
+      specialize (IHl₁ wfl₁).
+      eapply prf_weaken_conclusion_meta.
+      4: apply IHl₁.
+      all: wf_auto2.
+  Defined.
+
+  Lemma prf_reorder_iter_meta {Σ : Signature} Γ a b g l₁ l₂ (i : ProofInfo):
+    well_formed a ->
+    well_formed b ->
+    well_formed g ->
+    Pattern.wf l₁ ->
+    Pattern.wf l₂ ->
+    Γ ⊢i (fold_right patt_imp g (l₁ ++ [a;b] ++ l₂)) using i ->
+    Γ ⊢i (fold_right patt_imp g (l₁ ++ [b;a] ++ l₂)) using i.
+  Proof.
+    (* TODO we should have a function/lemma for creating these "meta" variants. *)
+    intros WFa WFb WFg Wfl1 Wfl2 H.
+    eapply MP.
+    2: { apply useBasicReasoning. apply prf_reorder_iter; wf_auto2. }
+    exact H.
+  Defined.
+  
+  Lemma A_impl_not_not_B_meta {Σ : Signature} Γ A B (i : ProofInfo) :
+    well_formed A ->
+    well_formed B ->
+    Γ ⊢i A ---> ! !B using i ->
+    Γ ⊢i A ---> B using i.
+  Proof.
+    intros WFA WFB H.
+    eapply MP.
+    2: { apply useBasicReasoning. apply A_impl_not_not_B; wf_auto2. }
+    exact H.
+  Defined.
+
+  Lemma pf_conj_elim_l {Σ : Signature} Γ A B :
+    well_formed A ->
+    well_formed B ->
+    Γ ⊢i A and B ---> A using BasicReasoning.
+  Proof.
+    intros WFA WFB. unfold patt_and. unfold patt_not at 1.
+
+    assert (Γ ⊢i (! A ---> (! A or ! B)) using BasicReasoning).
+    { apply disj_left_intro; wf_auto2. }
+
+    assert (Γ ⊢i ((! A or ! B) ---> (! A or ! B ---> ⊥) ---> ⊥) using BasicReasoning).
+    {
+      apply modus_ponens; wf_auto2.
+    }
+    assert (Γ ⊢i (! A ---> ((! A or ! B ---> ⊥) ---> ⊥)) using BasicReasoning).
+    { eapply syllogism_meta. 5: apply H0. 4: apply H. all: wf_auto2. }
+    epose proof (reorder_meta _ _ _ H1).
+    apply A_impl_not_not_B_meta;[wf_auto2|wf_auto2|].
+    apply H2.
+    Unshelve.
+    all: wf_auto2.
+  Defined.
+
+  Lemma pf_conj_elim_r {Σ : Signature} Γ A B :
+    well_formed A ->
+    well_formed B ->
+    Γ ⊢i A and B ---> B using BasicReasoning.
+  Proof.
+    intros WFA WFB. unfold patt_and. unfold patt_not at 1.
+
+    assert (Γ ⊢i (! B ---> (! A or ! B)) using BasicReasoning).
+    { apply disj_right_intro; wf_auto2. }
+
+    assert (Γ ⊢i ((! A or ! B) ---> (! A or ! B ---> ⊥) ---> ⊥) using BasicReasoning).
+    { apply modus_ponens; wf_auto2. }
+
+    assert (Γ ⊢i (! B ---> ((! A or ! B ---> ⊥) ---> ⊥)) using BasicReasoning).
+    { eapply syllogism_meta. 5: apply H0. 4: apply H. all: wf_auto2. }
+    epose proof (reorder_meta  _ _ _ H1).
+    apply A_impl_not_not_B_meta;[wf_auto2|wf_auto2|].
+    apply H2.
+    Unshelve.
+    all: wf_auto2.
+  Defined.
+
+  Lemma pf_conj_elim_l_meta {Σ : Signature} Γ A B (i : ProofInfo) :
+    well_formed A ->
+    well_formed B ->
+    Γ ⊢i A and B using i ->
+    Γ ⊢i A using i.
+  Proof.
+    intros WFA WFB H.
+    eapply MP.
+    2: { apply useBasicReasoning. apply pf_conj_elim_l. wf_auto2. shelve. }
+    1: apply H.
+    Unshelve. all: wf_auto2.
+  Defined.
+  
+  Lemma pf_conj_elim_r_meta {Σ : Signature} Γ A B (i : ProofInfo) :
+    well_formed A ->
+    well_formed B ->
+    Γ ⊢i A and B using i ->
+    Γ ⊢i B using i.
+  Proof.
+    intros WFA WFB H.
+    eapply MP.
+    2: apply useBasicReasoning; apply pf_conj_elim_r.
+    1: apply H.
+    all: wf_auto2.
+  Defined.
+
+  Lemma A_or_notA {Σ : Signature} Γ A :
+    well_formed A ->
+    Γ ⊢i A or ! A using BasicReasoning.
+  Proof.
+    intros wfA.
+    unfold patt_or.
+    apply A_impl_A. wf_auto2.
+  Defined.
+
+  Lemma P4m_meta {Σ : Signature} (Γ : Theory) (A B : Pattern) (i : ProofInfo) :
+    well_formed A ->
+    well_formed B ->
+    Γ ⊢i A ---> B using i ->
+    Γ ⊢i A ---> !B using i ->
+    Γ ⊢i !A using i.
+  Proof.
+    intros wfA wfB AimpB AimpnB.
+    pose proof (H1 := @P4m _ Γ A B wfA wfB).
+    assert (H2 : Γ ⊢i (A ---> ! B) ---> ! A using i).
+    { eapply MP. 2: { apply useBasicReasoning; apply H1. } exact AimpB. }
+    eapply MP. 2: { apply H2. } exact AimpnB.
+  Defined.
+
+
+Lemma MLGoal_exactn {Σ : Signature} (Γ : Theory) (l₁ l₂ : list Pattern) (g : Pattern):
+  @mkMLGoal Σ Γ (l₁ ++ g :: l₂) g BasicReasoning.
+Proof.
+  mlExtractWF wfl₁gl₂ wfg.
+  fromMLGoal.
+  apply nested_const_middle.
+  { exact wfg. }
+  { abstract (
+      pose proof (wfl₁ := wf_take (length l₁) wfl₁gl₂);
+      rewrite take_app in wfl₁;
+      exact wfl₁
+    ).
+  }
+  {
+    abstract (
+      pose proof (wfgl₂ := wf_drop (length l₁) wfl₁gl₂);
+      rewrite drop_app in wfgl₂;
+      unfold Pattern.wf in wfgl₂;
+      simpl in wfgl₂;
+      apply andb_prop in wfgl₂;
+      destruct wfgl₂ as [_ wfl₂];
+      exact wfl₂
+    ).
+  }
+Defined.
+
+Tactic Notation "mlExactn" constr(n) :=
+  useBasicReasoning;
+  unshelve (eapply (@cast_proof_ml_hyps _ _ _ _ _ _ _));
+  [shelve|(rewrite <- (firstn_skipn n); rewrite /firstn; rewrite /skipn; reflexivity)|idtac];
+  apply MLGoal_exactn.
+
+
+Local Example ex_mlExactn {Σ : Signature} Γ a b c:
+  well_formed a = true ->
+  well_formed b = true ->
+  well_formed c = true ->
+  Γ ⊢i a ---> b ---> c ---> b using BasicReasoning.
+Proof.
+  intros wfa wfb wfc.
+  toMLGoal.
+  { wf_auto2. }
+  mlIntro. mlIntro. mlIntro.
+  mlExactn 1.
+Defined.
+
+
+
+Lemma MLGoal_weakenConclusion' {Σ : Signature} Γ l g g' (i : ProofInfo):
+Γ ⊢i g ---> g' using i ->
+@mkMLGoal Σ Γ l g i ->
+@mkMLGoal Σ Γ l g' i.
+Proof.
+intros Hgg' Hlg.
+(*mlExtractWF wfl wfgp.*)
+unfold of_MLGoal in *. simpl in *.
+intros wfg' wfl.
+pose proof (wfimp := proved_impl_wf _ _ (proj1_sig Hgg')).
+apply well_formed_imp_proj1 in wfimp.
+eapply prf_weaken_conclusion_iter_meta_meta.
+5: apply Hlg.
+4: apply Hgg'.
+all: assumption.
+Defined.
+
+Lemma prf_contraction {Σ : Signature} Γ a b:
+well_formed a ->
+well_formed b ->
+Γ ⊢i ((a ---> a ---> b) ---> (a ---> b)) using BasicReasoning.
+Proof.
+intros wfa wfb.
+assert (H1 : Γ ⊢i (a ---> ((a ---> b) ---> b)) using BasicReasoning).
+{
+  apply modus_ponens; assumption.
+}
+assert (H2 : Γ ⊢i ((a ---> ((a ---> b) ---> b)) ---> ((a ---> (a ---> b)) ---> (a ---> b))) using BasicReasoning).
+{
+  apply P2; wf_auto2.
+}
+eapply MP. 2: apply H2. apply H1.
+Defined.
+
+Lemma prf_weaken_conclusion_under_implication {Σ : Signature} Γ a b c:
+well_formed a ->
+well_formed b ->
+well_formed c ->
+Γ ⊢i ((a ---> b) ---> ((a ---> (b ---> c)) ---> (a ---> c))) using BasicReasoning.
+Proof.
+intros wfa wfb wfc.
+assert (H1 : Γ ⊢i ((a ---> (b ---> c)) ---> (b ---> (a ---> c))) using BasicReasoning).
+{
+  apply reorder; wf_auto2.
+}
+assert (H2 : Γ ⊢i (((b ---> (a ---> c)) ---> (a ---> c)) ---> ((a ---> (b ---> c)) ---> (a ---> c))) using BasicReasoning).
+{
+  apply prf_strenghten_premise_meta;[wf_auto2|wf_auto2|wf_auto2|].
+  apply H1.
+}
+eapply prf_weaken_conclusion_meta_meta.
+4: apply H2. 1-3: wf_auto2. clear H1 H2.
+
+assert (H3 : Γ ⊢i ((a ---> b) ---> ((b ---> (a ---> c)) ---> (a ---> (a ---> c)))) using BasicReasoning).
+{
+  apply syllogism; wf_auto2.
+}
+assert (H4 : Γ ⊢i ((a ---> (a ---> c)) ---> (a ---> c)) using BasicReasoning).
+{
+  apply prf_contraction; wf_auto2.
+}
+assert (Hiter: ((a ---> b) ---> (b ---> a ---> c) ---> a ---> c)
+               = foldr patt_imp (a ---> c) [(a ---> b); (b ---> a ---> c)]) by reflexivity.
+
+eapply (@cast_proof' _ _ _ _ _ Hiter).
+
+eapply prf_weaken_conclusion_iter_meta_meta.
+5: apply H3. 4: apply H4. all: wf_auto2.
+Defined.
+
+Lemma prf_weaken_conclusion_under_implication_meta {Σ : Signature} Γ a b c (i : ProofInfo):
+well_formed a ->
+well_formed b ->
+well_formed c ->
+Γ ⊢i (a ---> b) using i ->
+Γ ⊢i ((a ---> (b ---> c)) ---> (a ---> c)) using i.
+Proof.
+intros wfa wfb wfc H.
+eapply MP.
+2: { useBasicReasoning. apply prf_weaken_conclusion_under_implication; wf_auto2. }
+exact H.
+Defined.
+
+Lemma prf_weaken_conclusion_under_implication_meta_meta {Σ : Signature} Γ a b c i:
+well_formed a ->
+well_formed b ->
+well_formed c ->
+Γ ⊢i a ---> b using i ->
+Γ ⊢i a ---> b ---> c using i ->
+Γ ⊢i a ---> c using i.
+Proof.
+intros wfa wfb wfc H1 H2.
+eapply MP.
+{ apply H2. }
+{ apply prf_weaken_conclusion_under_implication_meta.
+  4: { apply H1. }
+  all: wf_auto2.
+}
+Defined.
+
+Lemma prf_weaken_conclusion_iter_under_implication {Σ : Signature} Γ l g g':
+Pattern.wf l ->
+well_formed g ->
+well_formed g' ->
+Γ ⊢i (((g ---> g') ---> (foldr patt_imp g l)) ---> ((g ---> g') ---> (foldr patt_imp g' l)))
+using BasicReasoning.
+Proof.
+intros wfl wfg wfg'.
+pose proof (H1 := @prf_weaken_conclusion_iter Σ Γ l g g' wfl wfg wfg').
+remember ((g ---> g')) as a.
+remember (foldr patt_imp g l) as b.
+remember (foldr patt_imp g' l) as c.
+assert (well_formed a) by (subst; wf_auto2).
+assert (well_formed b) by (subst; wf_auto2).
+assert (well_formed c) by (subst; wf_auto2).
+pose proof (H2' := @prf_weaken_conclusion_under_implication _ Γ a b c ltac:(assumption) ltac:(assumption) ltac:(assumption)).
+apply reorder_meta in H2'. 2,3,4: subst;wf_auto2.
+eapply MP. 2: apply H2'. apply H1.
+Defined.
+
+Lemma prf_weaken_conclusion_iter_under_implication_meta {Σ : Signature} Γ l g g' (i : ProofInfo):
+Pattern.wf l ->
+well_formed g ->
+well_formed g' ->
+Γ ⊢i ((g ---> g') ---> (foldr patt_imp g l)) using i->
+Γ ⊢i ((g ---> g') ---> (foldr patt_imp g' l)) using i.
+Proof.
+intros wfl wfg wfg' H.
+eapply MP.
+2: { useBasicReasoning. apply prf_weaken_conclusion_iter_under_implication; wf_auto2. }
+{ exact H. }
+Defined.
+
+Lemma MLGoal_weakenConclusion_under_first_implication {Σ : Signature} Γ l g g' i:
+@mkMLGoal Σ Γ ((g ---> g') :: l) g i ->
+@mkMLGoal Σ Γ ((g ---> g') :: l) g' i .
+Proof.
+intros H. unfold of_MLGoal in *. simpl in *.
+intros wfg' wfgg'l.
+pose proof (Htmp := wfgg'l).
+unfold Pattern.wf in Htmp. simpl in Htmp. apply andb_prop in Htmp. destruct Htmp as [wfgg' wfl].
+apply well_formed_imp_proj1 in wfgg'. specialize (H wfgg' wfgg'l).
+apply prf_weaken_conclusion_iter_under_implication_meta; assumption.
+Defined.
+
+Lemma prf_weaken_conclusion_iter_under_implication_iter {Σ : Signature} Γ l₁ l₂ g g':
+Pattern.wf l₁ ->
+Pattern.wf l₂ ->
+well_formed g ->
+well_formed g' ->
+Γ ⊢i ((foldr patt_imp g (l₁ ++ (g ---> g') :: l₂)) --->
+     (foldr patt_imp g' (l₁ ++ (g ---> g') :: l₂)))
+using BasicReasoning.
+Proof.
+intros wfl₁ wfl₂ wfg wfg'.
+induction l₁; simpl.
+- apply prf_weaken_conclusion_iter_under_implication; auto.
+- pose proof (wfal₁ := wfl₁). unfold Pattern.wf in wfl₁. simpl in wfl₁. apply andb_prop in wfl₁.
+  destruct wfl₁ as [wfa wfl₁]. specialize (IHl₁ wfl₁).
+  eapply prf_weaken_conclusion_meta. 4: assumption. all: wf_auto2.
+Defined.
+
+Lemma prf_weaken_conclusion_iter_under_implication_iter_meta {Σ : Signature} Γ l₁ l₂ g g' i:
+Pattern.wf l₁ ->
+Pattern.wf l₂ ->
+well_formed g ->
+well_formed g' ->
+Γ ⊢i (foldr patt_imp g (l₁ ++ (g ---> g') :: l₂)) using i ->
+Γ ⊢i (foldr patt_imp g' (l₁ ++ (g ---> g') :: l₂)) using i.
+Proof.
+intros wfl₁ wfl₂ wfg wfg' H.
+eapply MP.
+{ apply H. }
+{ useBasicReasoning. apply prf_weaken_conclusion_iter_under_implication_iter; wf_auto2. }
+Defined.
+
+Lemma MLGoal_weakenConclusion {Σ : Signature} Γ l₁ l₂ g g' i:
+@mkMLGoal Σ Γ (l₁ ++ (g ---> g') :: l₂) g i ->
+@mkMLGoal Σ Γ (l₁ ++ (g ---> g') :: l₂) g' i.
+Proof.
+unfold of_MLGoal in *. simpl in *.
+intros H wfg' wfl₁gg'l₂.
+
+apply prf_weaken_conclusion_iter_under_implication_iter_meta.
+{ abstract (pose proof (wfl₁ := wf_take (length l₁) wfl₁gg'l₂); rewrite take_app in wfl₁; exact wfl₁). }
+{ abstract (
+    pose proof (wfgg'l₂ := wf_drop (length l₁) wfl₁gg'l₂);
+    rewrite drop_app in wfgg'l₂;
+    pose proof (Htmp := wfgg'l₂);
+    unfold Pattern.wf in Htmp;
+    simpl in Htmp;
+    apply andb_prop in Htmp;
+    destruct Htmp as [wfgg' wfl₂];
+    exact wfl₂
+  ).
+}
+{
+  abstract(
+    pose proof (wfgg'l₂ := wf_drop (length l₁) wfl₁gg'l₂);
+    rewrite drop_app in wfgg'l₂;
+    pose proof (Htmp := wfgg'l₂);
+    unfold Pattern.wf in Htmp;
+    simpl in Htmp;
+    apply andb_prop in Htmp;
+    destruct Htmp as [wfgg' wfl₂];
+    pose proof (wfg := well_formed_imp_proj1 wfgg');
+    exact wfg
+  ).
+}
+{ exact wfg'. }
+apply H.
+{
+  abstract(
+    pose proof (wfgg'l₂ := wf_drop (length l₁) wfl₁gg'l₂);
+    rewrite drop_app in wfgg'l₂;
+    pose proof (Htmp := wfgg'l₂);
+    unfold Pattern.wf in Htmp;
+    simpl in Htmp;
+    apply andb_prop in Htmp;
+    destruct Htmp as [wfgg' wfl₂];
+    pose proof (wfg := well_formed_imp_proj1 wfgg');
+    exact wfg
+  ).
+}
+exact wfl₁gg'l₂.
+Defined.
+
+
+Tactic Notation "mlApply" constr(n) :=
+  unshelve (eapply (@cast_proof_ml_hyps _ _ _ _ _ _ _));
+  [shelve|(rewrite <- (firstn_skipn n); rewrite /firstn; rewrite /skipn; reflexivity)|idtac];
+  apply MLGoal_weakenConclusion;
+  let hyps := fresh "hyps" in rewrite [hyps in @mkMLGoal _ _ hyps _]/app.
+
+Local Example ex_mlApply {Σ : Signature} Γ a b:
+  well_formed a ->
+  well_formed b ->
+  Γ ⊢i a ---> (a ---> b) ---> b using BasicReasoning.
+Proof.
+  intros wfa wfb.
+  toMLGoal.
+  { wf_auto2. }
+  mlIntro. mlIntro.
+  mlApply 1.
+  fromMLGoal. apply P1; wf_auto2.
+Defined.
+
+
+Lemma Constructive_dilemma {Σ : Signature} Γ p q r s:
+well_formed p ->
+well_formed q ->
+well_formed r ->
+well_formed s ->
+Γ ⊢i ((p ---> q) ---> (r ---> s) ---> (p or r) ---> (q or s)) using BasicReasoning.
+Proof.
+intros wfp wfq wfr wfs.
+unfold patt_or.
+
+toMLGoal.
+{ wf_auto2. }
+
+mlIntro. mlIntro. mlIntro. mlIntro.
+mlApply 1.
+mlApply 2.
+mlIntro.
+mlApply 3.
+mlApply 0.
+mlExactn 4.
+Defined.
+
+Lemma prf_add_assumption {Σ : Signature} Γ a b i :
+well_formed a ->
+well_formed b ->
+Γ ⊢i b using i ->
+Γ ⊢i (a ---> b) using i.
+Proof.
+intros wfa wfb H.
+eapply MP.
+{ apply H. }
+{ useBasicReasoning. apply P1; wf_auto2. }
+Defined.
+
+Lemma prf_impl_distr_meta {Σ : Signature} Γ a b c i:
+well_formed a ->
+well_formed b ->
+well_formed c ->
+Γ ⊢i (a ---> (b ---> c)) using i ->
+Γ ⊢i ((a ---> b) ---> (a ---> c)) using i.
+Proof.
+intros wfa wfb wfc H.
+eapply MP.
+{ apply H. }
+{ useBasicReasoning. apply P2; wf_auto2. }
+Defined.
+
+Lemma prf_add_lemma_under_implication {Σ : Signature} Γ l g h:
+Pattern.wf l ->
+well_formed g ->
+well_formed h ->
+Γ ⊢i ((foldr patt_imp h l) --->
+     ((foldr patt_imp g (l ++ [h])) --->
+      (foldr patt_imp g l)))
+using BasicReasoning.
+Proof.
+intros wfl wfg wfh.
+induction l; simpl.
+- apply modus_ponens; auto.
+- pose proof (wfal := wfl).
+  unfold Pattern.wf in wfl. apply andb_prop in wfl. destruct wfl as [wfa wfl].
+  specialize (IHl wfl).
+  assert (H1: Γ ⊢i a --->
+                  foldr patt_imp h l --->
+                  foldr patt_imp g (l ++ [h]) --->
+                  foldr patt_imp g l
+          using BasicReasoning).
+  { apply prf_add_assumption; wf_auto2. }
+
+  assert (H2 : Γ ⊢i (a ---> foldr patt_imp h l) --->
+                   (a ---> foldr patt_imp g (l ++ [h]) --->
+                   foldr patt_imp g l)
+          using BasicReasoning).
+  { apply prf_impl_distr_meta;[wf_auto2|wf_auto2|wf_auto2|]. apply H1. }
+
+  assert (H3 : Γ ⊢i ((a ---> foldr patt_imp g (l ++ [h]) ---> foldr patt_imp g l)
+                      ---> ((a ---> foldr patt_imp g (l ++ [h])) ---> (a ---> foldr patt_imp g l)))
+          using BasicReasoning).
+  { apply P2; wf_auto2. }
+
+  eapply prf_weaken_conclusion_meta_meta.
+  4: apply H3. 4: apply H2. all: wf_auto2.
+Defined.
+
+Lemma prf_add_lemma_under_implication_meta {Σ : Signature} Γ l g h i:
+Pattern.wf l ->
+well_formed g ->
+well_formed h ->
+Γ ⊢i (foldr patt_imp h l) using i ->
+Γ ⊢i ((foldr patt_imp g (l ++ [h])) ---> (foldr patt_imp g l)) using i.
+Proof.
+intros WFl WFg WGh H.
+eapply MP.
+{ apply H. }
+{ useBasicReasoning. apply prf_add_lemma_under_implication. all: wf_auto2. }
+Defined.
+
+Lemma prf_add_lemma_under_implication_meta_meta {Σ : Signature} Γ l g h i:
+Pattern.wf l ->
+well_formed g ->
+well_formed h ->
+Γ ⊢i (foldr patt_imp h l) using i ->
+Γ ⊢i (foldr patt_imp g (l ++ [h])) using i ->
+Γ ⊢i (foldr patt_imp g l) using i.
+Proof.
+intros WFl WFg WGh H H0.
+eapply MP.
+{ apply H0. }
+{ apply prf_add_lemma_under_implication_meta. 4: apply H. all: wf_auto2. }
+Defined.
+
+Lemma myGoal_assert {Σ : Signature} Γ l g h i:
+well_formed h ->
+@mkMLGoal Σ Γ l h i ->
+@mkMLGoal Σ Γ (l ++ [h]) g i ->
+@mkMLGoal Σ Γ l g i.
+Proof.
+intros wfh H1 H2.
+unfold of_MLGoal in *. simpl in *.
+intros wfg wfl.
+eapply prf_add_lemma_under_implication_meta_meta.
+4: apply H1. 6: apply H2. all: try assumption.
+{ abstract (
+    unfold Pattern.wf;
+    rewrite map_app;
+    rewrite foldr_app;
+    simpl;
+    rewrite wfh;
+    simpl;
+    exact wfl
+  ).
+}
+Defined.
+
+Lemma prf_add_lemma_under_implication_generalized {Σ : Signature} Γ l1 l2 g h:
+Pattern.wf l1 ->
+Pattern.wf l2 ->
+well_formed g ->
+well_formed h ->
+Γ ⊢i ((foldr patt_imp h l1) ---> ((foldr patt_imp g (l1 ++ [h] ++ l2)) ---> (foldr patt_imp g (l1 ++ l2))))
+using BasicReasoning.
+Proof.
+intros wfl1 wfl2 wfg wfh.
+induction l1; simpl.
+- apply modus_ponens; wf_auto2.
+- pose proof (wfal1 := wfl1).
+  unfold Pattern.wf in wfl1. simpl in wfl1. apply andb_prop in wfl1. destruct wfl1 as [wfa wfl1].
+  specialize (IHl1 wfl1).
+  assert (H1: Γ ⊢i a ---> foldr patt_imp h l1 ---> foldr patt_imp g (l1 ++ [h] ++ l2) ---> foldr patt_imp g (l1 ++ l2) using BasicReasoning).
+  { apply prf_add_assumption; wf_auto2. }
+  assert (H2 : Γ ⊢i (a ---> foldr patt_imp h l1) ---> (a ---> foldr patt_imp g (l1 ++ [h] ++ l2) ---> foldr patt_imp g (l1 ++ l2)) using BasicReasoning).
+  { apply prf_impl_distr_meta;[wf_auto2|wf_auto2|wf_auto2|]. exact H1. }
+  assert (H3 : Γ ⊢i ((a ---> foldr patt_imp g (l1 ++ [h] ++ l2) ---> foldr patt_imp g (l1 ++ l2))
+                      ---> ((a ---> foldr patt_imp g (l1 ++ [h] ++ l2)) ---> (a ---> foldr patt_imp g (l1 ++ l2)))) using BasicReasoning).
+  { apply P2; wf_auto2. }
+
+  eapply prf_weaken_conclusion_meta_meta.
+  4: apply H3. 4: assumption. all: wf_auto2.
+Defined.
+
+Lemma prf_add_lemma_under_implication_generalized_meta {Σ : Signature} Γ l1 l2 g h i:
+Pattern.wf l1 ->
+Pattern.wf l2 ->
+well_formed g ->
+well_formed h ->
+Γ ⊢i (foldr patt_imp h l1) using i ->
+Γ ⊢i ((foldr patt_imp g (l1 ++ [h] ++ l2)) ---> (foldr patt_imp g (l1 ++ l2))) using i.
+Proof.
+intros WFl1 WFl2 WFg WGh H.
+eapply MP.
+{ apply H. }
+{ useBasicReasoning.
+  apply prf_add_lemma_under_implication_generalized; wf_auto2.
+}
+Defined.
+
+Lemma prf_add_lemma_under_implication_generalized_meta_meta {Σ : Signature} Γ l1 l2 g h i:
+Pattern.wf l1 ->
+Pattern.wf l2 ->
+well_formed g ->
+well_formed h ->
+Γ ⊢i (foldr patt_imp h l1) using i ->
+Γ ⊢i (foldr patt_imp g (l1 ++ [h] ++ l2)) using i ->
+Γ ⊢i (foldr patt_imp g (l1 ++ l2)) using i.
+Proof.
+intros WFl1 WFl2 WFg WGh H H0.
+eapply MP.
+{ apply H0. }
+{ apply prf_add_lemma_under_implication_generalized_meta.
+  5: apply H. all: wf_auto2.
+}
+Defined.
+
+Lemma myGoal_assert_generalized {Σ : Signature} Γ l1 l2 g h i:
+well_formed h ->
+@mkMLGoal Σ Γ l1 h i ->
+@mkMLGoal Σ Γ (l1 ++ [h] ++ l2) g i ->
+@mkMLGoal Σ Γ (l1 ++ l2) g i.
+Proof.
+intros wfh H1 H2.
+unfold of_MLGoal in *. simpl in *.
+intros wfg wfl1l2.
+eapply prf_add_lemma_under_implication_generalized_meta_meta.
+5: apply H1. 7: apply H2. all: try assumption.
+{ abstract (
+      apply (wf_take (length l1)) in wfl1l2;
+      rewrite take_app in wfl1l2;
+      exact wfl1l2
+  ).
+}
+{ abstract (
+      apply (wf_drop (length l1)) in wfl1l2;
+      rewrite drop_app in wfl1l2;
+      exact wfl1l2
+  ).
+}
+{ abstract (
+      apply (wf_take (length l1)) in wfl1l2;
+      rewrite take_app in wfl1l2;
+      exact wfl1l2
+  ).
+}
+{
+  abstract(
+    pose proof (wfl1 := wf_take (length l1) wfl1l2);
+    rewrite take_app in wfl1;
+    pose proof (wfl2 := wf_drop (length l1) wfl1l2);
+    rewrite drop_app in wfl2;
+    unfold Pattern.wf; rewrite map_app; rewrite foldr_app;
+    simpl; rewrite wfh; unfold Pattern.wf in wfl2; rewrite wfl2;
+    simpl; exact wfl1
+  ).
+}
+Defined.
+
+
+
+Tactic Notation "mlAssert" "(" constr(t) ")" :=
+  match goal with
+  | |- @of_MLGoal ?Sgm (@mkMLGoal ?Sgm ?Ctx ?l ?g ?i) =>
+    let Hwf := fresh "Hwf" in
+    assert (Hwf : well_formed t);
+    [idtac|
+      let H := fresh "H" in
+      assert (H : @mkMLGoal Sgm Ctx l t i);
+      [ | (eapply (@myGoal_assert Sgm Ctx l g t i Hwf H); rewrite [_ ++ _]/=; clear H)]
+    ]
+  end.
+
+Local Example ex_mlAssert {Σ : Signature} Γ a:
+  well_formed a ->
+  Γ ⊢i (a ---> a ---> a) using BasicReasoning.
+Proof.
+  intros wfa.
+  toMLGoal.
+  { wf_auto2. }
+  mlIntro. mlIntro.
+  mlAssert (a).
+  { wf_auto2. }
+  { mlExactn 1. }
+  { mlExactn 2. }
+Qed.
+
+Tactic Notation "mlAssert" "(" constr(t) ")" "using" "first" constr(n) :=
+  lazymatch goal with
+  | |- @of_MLGoal ?Sgm (@mkMLGoal ?Sgm ?Ctx ?l ?g ?i) =>
+    let l1 := fresh "l1" in
+    let l2 := fresh "l2" in
+    let Heql1 := fresh "Heql1" in
+    let Heql2 := fresh "Heql2" in
+    remember (take n l) as l1 eqn:Heql1 in |-;
+    remember (drop n l) as l2 eqn:Heql2 in |-;
+    simpl in Heql1; simpl in Heql2;
+    eapply cast_proof_ml_hyps;
+    [(
+      rewrite -[l](take_drop n);
+      reflexivity
+     )|];
+    let Hwf := fresh "Hwf" in
+    assert (Hwf : well_formed t);
+    [idtac|
+      let H := fresh "H" in
+      assert (H : @mkMLGoal Sgm Ctx l1 t i) ;
+      [
+        (eapply cast_proof_ml_hyps; [(rewrite Heql1; reflexivity)|]);  clear l1 l2 Heql1 Heql2
+      | apply (cast_proof_ml_hyps Heql1) in H;
+        eapply (@myGoal_assert_generalized Sgm Ctx (take n l) (drop n l) g t i Hwf H);
+        rewrite [_ ++ _]/=; clear l1 l2 Heql1 Heql2 H] 
+    ]
+  end.
+
+Local Example ex_assert_using {Σ : Signature} Γ p q a b:
+  well_formed a = true ->
+  well_formed b = true ->
+  well_formed p = true ->
+  well_formed q = true ->
+  Γ ⊢i a ---> p and q ---> b ---> ! ! q using BasicReasoning.
+Proof.
+  intros wfa wfb wfp wfq.
+  toMLGoal.
+  { wf_auto2. }
+  do 3 mlIntro.
+  mlAssert (p) using first 2.
+  { wf_auto2. }
+  { admit. }
+  { admit. }
+Abort.
+
+
+
+Lemma P4i' {Σ : Signature} (Γ : Theory) (A : Pattern) :
+well_formed A →
+Γ ⊢i ((!A ---> A) ---> A) using BasicReasoning.
+Proof.
+intros wfA.
+assert (H1: Γ ⊢i ((! A ---> ! ! A) ---> ! ! A) using BasicReasoning).
+{ apply P4i. wf_auto2. }
+assert (H2: Γ ⊢i ((! A ---> A) ---> (! A ---> ! ! A)) using BasicReasoning).
+{ eapply prf_weaken_conclusion_meta. 
+  4: apply not_not_intro.
+  all: wf_auto2.
+}
+
+eapply prf_strenghten_premise_meta_meta. 4: apply H2.
+4: eapply prf_weaken_conclusion_meta_meta. 7: apply not_not_elim.
+8: { apply H1. }
+all: wf_auto2.
+Defined.
+
+Lemma tofold {Σ : Signature} p:
+p = fold_right patt_imp p [].
+Proof.
+reflexivity.
+Defined.
+
+Lemma consume {Σ : Signature} p q l:
+fold_right patt_imp (p ---> q) l = fold_right patt_imp q (l ++ [p]).
+Proof.
+rewrite foldr_app. reflexivity.
+Defined.
+
+Lemma prf_disj_elim {Σ : Signature} Γ p q r:
+well_formed p ->
+well_formed q ->
+well_formed r ->
+Γ ⊢i ((p ---> r) ---> (q ---> r) ---> (p or q) ---> r)
+using BasicReasoning.
+Proof.
+intros wfp wfq wfr.
+pose proof (H1 := @Constructive_dilemma Σ Γ p r q r wfp wfr wfq wfr).
+assert (Γ ⊢i ((r or r) ---> r) using BasicReasoning).
+{ unfold patt_or. apply P4i'. wf_auto2. }
+eapply cast_proof' in H1.
+2: { rewrite -> tofold. do 3 rewrite -> consume. reflexivity. }
+eapply prf_weaken_conclusion_iter_meta_meta in H1. 5: apply H.
+{ apply H1. }
+all: wf_auto2.
+Defined.
+
+Lemma prf_disj_elim_meta {Σ : Signature} Γ p q r i:
+well_formed p ->
+well_formed q ->
+well_formed r ->
+Γ ⊢i (p ---> r) using i ->
+Γ ⊢i ((q ---> r) ---> (p or q) ---> r) using i.
+Proof.
+intros WFp WHq WFr H.
+eapply MP. apply H. useBasicReasoning. apply prf_disj_elim.
+all: wf_auto2.
+Defined.
+
+Lemma prf_disj_elim_meta_meta {Σ : Signature} Γ p q r i:
+well_formed p ->
+well_formed q ->
+well_formed r ->
+Γ ⊢i (p ---> r) using i ->
+Γ ⊢i (q ---> r) using i ->
+Γ ⊢i ((p or q) ---> r) using i.
+Proof.
+intros WFp WHq WFr H H0.
+eapply MP. apply H0. apply prf_disj_elim_meta. 4: apply H.
+all: wf_auto2.
+Defined.
+
+Lemma prf_disj_elim_meta_meta_meta {Σ : Signature} Γ p q r i:
+well_formed p ->
+well_formed q ->
+well_formed r ->
+Γ ⊢i (p ---> r) using i ->
+Γ ⊢i (q ---> r) using i ->
+Γ ⊢i (p or q) using i ->
+Γ ⊢i r using i.
+Proof.
+intros WFp WHq WFr H H0 H1.
+eapply MP. apply H1.
+apply prf_disj_elim_meta_meta.
+all: assumption.
+Defined.
+
+Lemma prf_add_proved_to_assumptions {Σ : Signature} Γ l a g i:
+Pattern.wf l ->
+well_formed a ->
+well_formed g ->
+Γ ⊢i a using i->
+Γ ⊢i ((foldr patt_imp g (a::l)) ---> (foldr patt_imp g l)) using i.
+Proof.
+intros wfl wfa wfg Ha.
+induction l.
+- simpl.
+  pose proof (@modus_ponens Σ Γ _ _ wfa wfg).
+  eapply MP. apply Ha. useBasicReasoning. apply H.
+- pose proof (wfa0l := wfl).
+  unfold Pattern.wf in wfl. simpl in wfl. apply andb_prop in wfl. destruct wfl as [wfa0 wfl].
+  specialize (IHl wfl).
+  simpl in IHl. simpl.
+  (* < change a0 and a in the LHS > *)
+  assert (H : Γ ⊢i (a ---> a0 ---> foldr patt_imp g l) ---> (a0 ---> a ---> foldr patt_imp g l) using BasicReasoning).
+  { apply reorder; wf_auto2. }
+
+  eapply cast_proof'.
+  { rewrite -> tofold. rewrite -> consume. reflexivity. }
+  pose proof (H0 := @prf_strenghten_premise_iter_meta_meta Σ Γ [] []).
+  simpl in H0. simpl.
+  specialize (H0 (a0 ---> a ---> foldr patt_imp g l) (a ---> a0 ---> foldr patt_imp g l)).
+  specialize (H0 (a0 ---> foldr patt_imp g l)). simpl in H0. simpl.
+  simpl. apply H0. all: try_wfauto2.
+  { useBasicReasoning. apply H. }
+  clear H0 H.
+  (* </change a0 and a > *)
+  assert (Γ ⊢i ((a ---> a0 ---> foldr patt_imp g l) ---> (a0 ---> foldr patt_imp g l)) using i).
+  { eapply MP. 2: { useBasicReasoning. apply modus_ponens; wf_auto2. } apply Ha. }
+  
+  eapply prf_strenghten_premise_meta_meta. 5: apply H. all: try_wfauto2.
+  useBasicReasoning.
+  apply reorder; wf_auto2.
+Defined.
+
+Lemma prf_add_proved_to_assumptions_meta {Σ : Signature} Γ l a g i:
+Pattern.wf l ->
+well_formed a ->
+well_formed g ->
+Γ ⊢i a using i ->
+Γ ⊢i (foldr patt_imp g (a::l)) using i ->
+Γ ⊢i (foldr patt_imp g l) using i.
+Proof.
+intros WFl WFa WFg H H0.
+eapply MP.
+apply H0.
+eapply prf_add_proved_to_assumptions.
+4: apply H.
+all: wf_auto2.
+Defined.
+
+Lemma MLGoal_add {Σ : Signature} Γ l g h i:
+Γ ⊢i h using i ->
+@mkMLGoal Σ Γ (h::l) g i ->
+@mkMLGoal Σ Γ l g i.
+Proof.
+intros H H0.
+unfold of_MLGoal in *. simpl in *.
+intros wfg wfl.
+apply prf_add_proved_to_assumptions_meta with (a := h).
+5: apply H0.
+all: try assumption.
+{ abstract (pose (tmp := proj1_sig H); apply proved_impl_wf in tmp; exact tmp). }
+{ abstract (
+      unfold Pattern.wf;
+      simpl;
+      pose (tmp := proj1_sig H);
+      apply proved_impl_wf in tmp;
+      rewrite tmp;
+      simpl;
+      exact wfl
+  ).
+}
+Defined.
+
+Tactic Notation "mlAdd" constr(n) :=
+  match goal with
+  | |- @of_MLGoal ?Sgm (@mkMLGoal ?Sgm ?Ctx ?l ?g ?i) =>
+    apply (@MLGoal_add Sgm Ctx l g _ i n)
+  end.
+
+
+  Local Example ex_mlAdd {Σ : Signature} Γ l g h i:
+    Pattern.wf l ->
+    well_formed g ->
+    well_formed h ->
+    Γ ⊢i (h ---> g) using i ->
+    Γ ⊢i h using i ->
+    Γ ⊢i g using i.
+  Proof.
+    intros WFl WFg WFh H H0. toMLGoal.
+    { wf_auto2. }
+    mlAdd H0.
+    mlAdd H.
+    mlApply 0.    
+    mlExactn 1.
+  Defined.
+
+
+  Lemma prf_clear_hyp {Σ : Signature} Γ l1 l2 g h:
+    Pattern.wf l1 ->
+    Pattern.wf l2 ->
+    well_formed g ->
+    well_formed h ->
+    Γ ⊢i (foldr patt_imp g (l1 ++ l2)) ---> (foldr patt_imp g (l1 ++ [h] ++ l2))
+    using BasicReasoning.
+  Proof.
+    intros wfl1 wfl2 wfg wfh.
+    induction l1; simpl.
+    - apply P1; wf_auto2.
+    - unfold Pattern.wf in wfl1. simpl in wfl1. apply andb_prop in wfl1. destruct wfl1 as [wfa wfl1].
+      specialize (IHl1 wfl1).
+
+      assert (H1: Γ ⊢i a ---> foldr patt_imp g (l1 ++ l2) ---> foldr patt_imp g (l1 ++ [h] ++ l2) using BasicReasoning).
+      {
+        toMLGoal.
+        { wf_auto2. }
+        mlAdd IHl1.
+        mlIntro. mlExactn 0.
+      }
+      apply prf_impl_distr_meta; try_wfauto2. apply H1.
+  Defined.
+
+  Lemma prf_clear_hyp_meta {Σ : Signature} Γ l1 l2 g h i:
+    Pattern.wf l1 ->
+    Pattern.wf l2 ->
+    well_formed g ->
+    well_formed h ->
+    Γ ⊢i (foldr patt_imp g (l1 ++ l2)) using i ->
+    Γ ⊢i (foldr patt_imp g (l1 ++ [h] ++ l2)) using i.
+  Proof.
+    intros. eapply MP.
+    apply H3.
+    useBasicReasoning.
+    apply prf_clear_hyp; wf_auto2.
+  Defined.  
+
+  
+
+  Lemma myGoal_clear_hyp {Σ : Signature} Γ l1 l2 g h i:
+    @mkMLGoal Σ Γ (l1 ++ l2) g i ->
+    @mkMLGoal Σ Γ (l1 ++ h::l2) g i.
+  Proof.
+    intros H1.
+    unfold of_MLGoal in *. simpl in *. intros wfg wfl1hl2.
+    apply prf_clear_hyp_meta.
+    5: apply H1. all: try assumption.
+    { apply wfl₁hl₂_proj_l₁ in wfl1hl2. exact wfl1hl2. }
+    { apply wfl₁hl₂_proj_l₂ in wfl1hl2. exact wfl1hl2. }
+    { apply wfl₁hl₂_proj_h in wfl1hl2. exact wfl1hl2. }
+    { apply wfl₁hl₂_proj_l₁l₂ in wfl1hl2. exact wfl1hl2. }
+  Defined.
+  
+
+
+Tactic Notation "mlClear" constr(n) :=
+match goal with
+| |- @of_MLGoal ?Sgm (@mkMLGoal ?Sgm ?Ctx ?l ?g ?i) =>
+  let l1 := fresh "l1" in
+  let l2 := fresh "l2" in
+  let Heql1 := fresh "Heql1" in
+  let Heql2 := fresh "Heql2" in
+  eapply cast_proof_ml_hyps;
+  [(rewrite -[l](take_drop n); reflexivity)|];
+  remember (take n l) as l1 eqn:Heql1 in |-;
+  remember (drop n l) as l2 eqn:Heql2 in |-;
+  eapply cast_proof_ml_hyps;
+  [(rewrite -Heql1; rewrite -Heql2; reflexivity)|];
+  simpl in Heql1; simpl in Heql2;
+  let a := fresh "a" in
+  let Hd := fresh "Hd" in
+  destruct l2 as [|a l2''] eqn:Hd in *|-;[congruence|];
+  eapply cast_proof_ml_hyps;
+  [(rewrite -> Hd at 1; reflexivity)|];
+  let Heqa := fresh "Heqa" in
+  let Heql2' := fresh "Heql2'" in
+  inversion Heql2 as [[Heqa Heql2'] ]; clear Heql2;
+  apply myGoal_clear_hyp;
+  eapply cast_proof_ml_hyps;
+  [(try(rewrite -> Heql1 at 1); try(rewrite -> Heql2' at 1); reflexivity)|];
+  clear Hd Heql2' Heqa l2 l2'' a Heql1 l1;
+  eapply cast_proof_ml_hyps;[rewrite {1}[_ ++ _]/=; reflexivity|]
+end.
+
+Local Example ex_mlClear {Σ : Signature} Γ a b c:
+well_formed a ->
+well_formed b ->
+well_formed c ->
+Γ ⊢i a ---> (b ---> (c ---> b)) using BasicReasoning.
+Proof.
+intros wfa wfb wfc.
+toMLGoal.
+{ wf_auto2. }
+repeat mlIntro.
+mlClear 2.
+mlClear 0.
+mlExactn 0.
+Defined.
+
+
+Lemma not_concl {Σ : Signature} Γ p q:
+well_formed p ->
+well_formed q ->
+Γ ⊢i (p ---> (q ---> ((p ---> ! q) ---> ⊥))) using BasicReasoning.
+Proof.
+intros wfp wfq.
+eapply cast_proof'.
+{
+  rewrite [(p ---> q ---> (p ---> ! q) ---> ⊥)]tofold.
+  do 3 rewrite consume.
+  rewrite [(((nil ++ [p]) ++ [q]) ++ [p ---> ! q])]/=.
+  replace ([p; q; p--->!q]) with ([p] ++ [q; p ---> !q] ++ []) by reflexivity.
+  reflexivity.
+}
+apply prf_reorder_iter_meta; try_wfauto2.
+simpl.
+fold (! q).
+apply modus_ponens; wf_auto2.
+Defined.
+
+(* TODO rename or remove *)
+Lemma helper {Σ : Signature} Γ p q r:
+well_formed p ->
+well_formed q ->
+well_formed r ->
+Γ ⊢i (p ---> (q ---> ((p ---> (q ---> r)) ---> r))) using BasicReasoning.
+Proof.
+intros wfp wfq wfr.
+eapply cast_proof'.
+{
+  rewrite [(p ---> q ---> (p ---> q ---> r) ---> r)]tofold. repeat rewrite consume.
+  replace ((([] ++ [p]) ++ [q]) ++ [p ---> (q ---> r)]) with ([p;q;p--->(q ---> r)]) by reflexivity.
+  replace ([p;q;p--->(q ---> r)]) with ([p] ++ [q; p ---> (q ---> r)] ++ []) by reflexivity.
+  reflexivity.
+}
+apply prf_reorder_iter_meta; try_wfauto2.
+simpl.
+apply modus_ponens; wf_auto2.
+Defined.
+
+Lemma reorder_last_to_head {Σ : Signature} Γ g x l:
+Pattern.wf l ->
+well_formed g ->
+well_formed x ->
+Γ ⊢i ((foldr patt_imp g (x::l)) ---> (foldr patt_imp g (l ++ [x]))) using BasicReasoning.
+Proof.
+intros wfl wfg wfx.
+induction l.
+- simpl. apply A_impl_A. wf_auto2.
+- pose proof (wfal := wfl).
+  unfold Pattern.wf in wfl. simpl in wfl. apply andb_prop in wfl. destruct wfl as [wfa wfl].
+  specialize (IHl wfl).
+  simpl. simpl in IHl.
+  eapply cast_proof'.
+  { rewrite -> tofold at 1. repeat rewrite -> consume. reflexivity. }
+  eapply prf_weaken_conclusion_iter_meta_meta.
+  4: { apply IHl. }
+  all: try_wfauto2.
+  eapply cast_proof'.
+  {
+    rewrite consume.
+    replace ((([] ++ [x ---> a ---> foldr patt_imp g l]) ++ [a]) ++ [x])
+      with ([x ---> a ---> foldr patt_imp g l] ++ [a;x] ++ []) by reflexivity.
+    reflexivity.
+  }
+  apply prf_reorder_iter_meta; wf_auto2.
+  simpl. apply A_impl_A. wf_auto2.
+Defined.
+
+Lemma reorder_last_to_head_meta {Σ : Signature} Γ g x l i:
+Pattern.wf l ->
+well_formed g ->
+well_formed x ->
+Γ ⊢i (foldr patt_imp g (x::l)) using i ->
+Γ ⊢i (foldr patt_imp g (l ++ [x])) using i.
+Proof.
+intros WFl WFG WFx H.
+eapply MP.
+apply H.
+useBasicReasoning.
+apply reorder_last_to_head; wf_auto2.
+Defined.
+
+(* Iterated modus ponens.
+ For l = [x₁, ..., xₙ], it says that
+ Γ ⊢i ((x₁ -> ... -> xₙ -> (x₁ -> ... -> xₙ -> r)) -> r)
+*)
+Lemma modus_ponens_iter {Σ : Signature} Γ l r:
+Pattern.wf l ->
+well_formed r ->
+Γ ⊢i (foldr patt_imp r (l ++ [foldr patt_imp r l])) using BasicReasoning.
+Proof.
+intros wfl wfr.
+induction l.
+- simpl. apply A_impl_A. exact wfr.
+- pose proof (wfal := wfl).
+  unfold Pattern.wf in wfl. simpl in wfl. apply andb_prop in wfl. destruct wfl as [wfa wfl].
+  specialize (IHl wfl).
+  simpl.
+  eapply cast_proof'.
+  { rewrite foldr_app. simpl. rewrite consume. simpl. reflexivity. }
+  eapply cast_proof' in IHl.
+  2: { rewrite foldr_app. reflexivity. }
+  simpl in IHl.
+  eapply prf_weaken_conclusion_meta_meta.
+  4: { apply reorder_last_to_head; wf_auto2. }
+  all: try_wfauto2.
+  simpl. apply modus_ponens; wf_auto2.
+Defined.
+
+Lemma and_impl {Σ : Signature} Γ p q r:
+well_formed p ->
+well_formed q ->
+well_formed r ->
+Γ ⊢i ((p and q ---> r) ---> (p ---> (q ---> r))) using BasicReasoning.
+Proof.
+intros wfp wfq wfr.
+toMLGoal.
+{ wf_auto2. }
+repeat mlIntro.
+unfold patt_and. mlApply 0.
+mlIntro. unfold patt_or at 2.
+mlAssert ((! ! p)).
+{ wf_auto2. }
+{
+  mlAdd (@not_not_intro Σ Γ p wfp).
+  mlApply 0.
+  mlExactn 2.
+}
+mlAssert ((! q)).
+{ wf_auto2. }
+{
+  mlApply 3. mlExactn 4.
+}
+mlApply 5. mlExactn 2.
+Defined.
+
+Lemma and_impl' {Σ : Signature} Γ p q r:
+well_formed p ->
+well_formed q ->
+well_formed r ->
+Γ ⊢i ((p ---> (q ---> r)) ---> ((p and q) ---> r)) using BasicReasoning.
+Proof.
+intros wfp wfq wfr.
+toMLGoal.
+{ wf_auto2. }
+repeat mlIntro.
+mlAssert (p).
+{ wf_auto2. }
+{
+  mlAdd (@pf_conj_elim_l Σ Γ p q wfp wfq).
+  mlApply 0.
+  mlExactn 2.
+}
+mlAssert (q).
+{ wf_auto2. }
+{
+  mlAdd (@pf_conj_elim_r Σ Γ p q wfp wfq).
+  mlApply 0.
+  mlExactn 2.
+}
+(* This pattern is basically an "apply ... in" *)
+mlAssert ((q ---> r)).
+{ wf_auto2. }
+{ mlApply 0. mlExactn 2. }
+mlApply 4. mlExactn 3.
+Defined.
+
+Lemma prf_disj_elim_iter {Σ : Signature} Γ l p q r:
+Pattern.wf l ->
+well_formed p ->
+well_formed q ->
+well_formed r ->
+Γ ⊢i ((fold_right patt_imp r (l ++ [p]))
+       --->
+       ((fold_right patt_imp r (l ++ [q]))
+          --->                                                                
+          (fold_right patt_imp r (l ++ [p or q]))))
+using BasicReasoning.
+Proof.
+intros wfl wfp wfq wfr.
+induction l.
+- simpl. apply prf_disj_elim; wf_auto2.
+- pose proof (wfal := wfl).
+  unfold Pattern.wf in wfl. simpl in wfl. apply andb_prop in wfl. destruct wfl as [wfa wfl].
+  specialize (IHl wfl).
+  simpl in *.
+  toMLGoal.
+  { wf_auto2. }
+  repeat mlIntro.
+  mlAdd IHl.
+  mlAssert ((foldr patt_imp r (l ++ [p]))).
+  { wf_auto2. }
+  { mlApply 1. mlExactn 3. }
+  mlAssert ((foldr patt_imp r (l ++ [q]))).
+  { wf_auto2. }
+  { mlApply 2. mlExactn 3. }
+  mlAssert ((foldr patt_imp r (l ++ [q]) ---> foldr patt_imp r (l ++ [p or q]))).
+  { wf_auto2. }
+  { mlApply 0. mlExactn 4. }
+  mlApply 6.
+  mlExactn 5.
+Defined.
+
+Lemma prf_disj_elim_iter_2 {Σ : Signature} Γ l₁ l₂ p q r:
+Pattern.wf l₁ ->
+Pattern.wf l₂ ->
+well_formed p ->
+well_formed q ->
+well_formed r ->
+Γ ⊢i ((fold_right patt_imp r (l₁ ++ [p] ++ l₂))
+       --->
+       ((fold_right patt_imp r (l₁ ++ [q] ++ l₂))
+          --->                                                                
+          (fold_right patt_imp r (l₁ ++ [p or q] ++ l₂))))
+using BasicReasoning.  
+Proof.
+intros wfl₁ wfl₂ wfp wfq wfr.
+move: l₁ wfl₁.
+induction l₂; intros l₁ wfl₁.
+- simpl. apply prf_disj_elim_iter; wf_auto2.
+- pose proof (wfal₂ := wfl₂).
+  unfold Pattern.wf in wfl₂. simpl in wfl₂. apply andb_prop in wfl₂. destruct wfl₂ as [wfa wfl₂].
+
+  simpl. (* We need to move 'a' to the beginning of l₁; then we can apply IHl₂. *)
+  (* Or we can swap p and a (move a to the end of l_1) *)
+  remember (foldr patt_imp r (l₁ ++ p :: a :: l₂)) as A in |-.
+  remember (foldr patt_imp r (l₁ ++ q :: a :: l₂)) as B in |-.
+  remember (foldr patt_imp r (l₁ ++ (p or q) :: a :: l₂)) as C in |-.
+  eapply cast_proof'.
+  { rewrite -HeqA. rewrite -HeqB. rewrite -HeqC. reflexivity. }
+  eapply cast_proof'.
+  {
+    rewrite -> tofold at 1. rewrite consume. rewrite consume. rewrite [_ ++ [B] ]/=.
+    rewrite -> HeqA at 1. rewrite -> HeqB at 1. rewrite -> HeqC at 1.
+    reflexivity.
+  }
+  eapply prf_weaken_conclusion_iter_meta_meta.
+  4: {
+    eapply cast_proof'.
+    {
+      replace (l₁ ++ (p or q) :: a :: l₂) with (l₁ ++ [p or q; a] ++ l₂) by reflexivity.
+      reflexivity.
+    }
+    apply prf_reorder_iter; wf_auto2.
+  }
+  all: try_wfauto2.
+  simpl.
+
+  eapply cast_proof'.
+  { 
+    rewrite -> tofold at 1. repeat rewrite consume. rewrite [_ ++ [_] ]/=.
+
+  replace
+    ([foldr patt_imp r (l₁ ++ p :: a :: l₂); foldr patt_imp r (l₁ ++ q :: a :: l₂)])
+    with
+      ([foldr patt_imp r (l₁ ++ p :: a :: l₂)] ++ (foldr patt_imp r (l₁ ++ q :: a :: l₂))::[])
+    by reflexivity.
+    reflexivity.
+  }
+
+  eapply prf_strenghten_premise_iter_meta_meta with (h := foldr patt_imp r (l₁ ++ a :: q :: l₂)).
+  6: { apply prf_reorder_iter; wf_auto2. }
+  all: try_wfauto2.
+
+  eapply cast_proof'.
+  {
+    replace
+      ([foldr patt_imp r (l₁ ++ p :: a :: l₂)] ++ [foldr patt_imp r (l₁ ++ a :: q :: l₂)])
+      with
+      ([] ++ ((foldr patt_imp r (l₁ ++ p :: a :: l₂))::[foldr patt_imp r (l₁ ++ a :: q :: l₂)]))
+      by reflexivity.
+    reflexivity.
+ }
+
+  eapply prf_strenghten_premise_iter_meta_meta with (h := (foldr patt_imp r (l₁ ++ a :: p :: l₂))).
+  6: {  apply prf_reorder_iter; wf_auto2. }
+  all: try_wfauto2.
+
+  simpl.
+  eapply cast_proof'.
+  {
+    replace (l₁ ++ a :: p :: l₂) with ((l₁ ++ [a]) ++ [p] ++ l₂) by (rewrite <- app_assoc; reflexivity).
+    replace (l₁ ++ a :: q :: l₂) with ((l₁ ++ [a]) ++ [q] ++ l₂) by (rewrite <- app_assoc; reflexivity).
+    replace (l₁ ++ a :: (p or q) :: l₂) with ((l₁ ++ [a]) ++ [p or q] ++ l₂) by (rewrite <- app_assoc; reflexivity).
+    reflexivity.
+  }
+  apply IHl₂; wf_auto2.
+Defined.
+
+Lemma prf_disj_elim_iter_2_meta {Σ : Signature} Γ l₁ l₂ p q r i:
+Pattern.wf l₁ ->
+Pattern.wf l₂ ->
+well_formed p ->
+well_formed q ->
+well_formed r ->
+Γ ⊢i (fold_right patt_imp r (l₁ ++ [p] ++ l₂)) using i ->
+Γ ⊢i ((fold_right patt_imp r (l₁ ++ [q] ++ l₂))
+          --->                                                                
+          (fold_right patt_imp r (l₁ ++ [p or q] ++ l₂))) using i.
+        
+Proof.
+intros WFl1 WFl2 WFp WFq WFr H.
+eapply MP.
+apply H.
+useBasicReasoning.
+apply prf_disj_elim_iter_2; wf_auto2.
+Defined.
+
+Lemma prf_disj_elim_iter_2_meta_meta {Σ : Signature} Γ l₁ l₂ p q r i:
+Pattern.wf l₁ ->
+Pattern.wf l₂ ->
+well_formed p ->
+well_formed q ->
+well_formed r ->
+Γ ⊢i (fold_right patt_imp r (l₁ ++ [p] ++ l₂)) using i ->
+Γ ⊢i (fold_right patt_imp r (l₁ ++ [q] ++ l₂)) using i ->
+Γ ⊢i (fold_right patt_imp r (l₁ ++ [p or q] ++ l₂)) using i.
+Proof.
+intros WFl1 WFl2 WFp WFq WFr H H0.
+eapply MP.
+2: { apply prf_disj_elim_iter_2_meta; try_wfauto2. apply H. }
+apply H0.
+Defined.
+
+Lemma MLGoal_disj_elim {Σ : Signature} Γ l₁ l₂ p q r i:
+@mkMLGoal Σ Γ (l₁ ++ [p] ++ l₂) r i ->
+@mkMLGoal Σ Γ (l₁ ++ [q] ++ l₂) r i ->
+@mkMLGoal Σ Γ (l₁ ++ [p or q] ++ l₂) r i.
+Proof.
+intros H1 H2.
+unfold of_MLGoal in *. simpl in *.
+intros wfr Hwf.
+apply prf_disj_elim_iter_2_meta_meta.
+7: apply H2.
+6: apply H1.
+all: try assumption.
+{ abstract (apply wfl₁hl₂_proj_l₁ in Hwf; exact Hwf). }
+{ abstract (apply wfl₁hl₂_proj_l₂ in Hwf; exact Hwf). }
+{ abstract (apply wfl₁hl₂_proj_h in Hwf; wf_auto2). }
+{ abstract (apply wfl₁hl₂_proj_h in Hwf; wf_auto2). }
+{ abstract (
+    pose proof (wfl₁hl₂_proj_l₁ Hwf);
+    pose proof (wfl₁hl₂_proj_h Hwf);
+    pose proof (wfl₁hl₂_proj_l₂ Hwf);
+    apply wf_app; [assumption|];
+    unfold patt_or,patt_not in *;
+    wf_auto2
+  ).
+}
+{ abstract (
+    pose proof (wfl₁hl₂_proj_l₁ Hwf);
+    pose proof (wfl₁hl₂_proj_h Hwf);
+    pose proof (wfl₁hl₂_proj_l₂ Hwf);
+    apply wf_app; [assumption|];
+    unfold patt_or,patt_not in *;
+    wf_auto2
+  ).
+}
+Defined.
+
+Tactic Notation "mlDestructOr" constr(n) :=
+  match goal with
+  | |- @of_MLGoal ?Sgm (@mkMLGoal ?Sgm ?Ctx ?l ?g ?i) =>
+    let Htd := fresh "Htd" in
+    eapply cast_proof_ml_hyps;
+    [(
+      epose proof (Htd :=take_drop);
+      specialize (Htd n l);
+      rewrite [take _ _]/= in Htd;
+      rewrite [drop _ _]/= in Htd;
+      rewrite -Htd; clear Htd;
+      epose proof (Htd :=take_drop);
+      specialize (Htd 1 (drop n l));
+      rewrite [take _ _]/= in Htd;
+      rewrite ![drop _ _]/= in Htd;
+      rewrite -Htd; clear Htd; reflexivity
+      )|];
+    apply MLGoal_disj_elim; simpl
+  end.
+
+  Local Example exd {Σ : Signature} Γ a b p q c i:
+  well_formed a ->
+  well_formed b ->
+  well_formed p ->
+  well_formed q ->
+  well_formed c ->
+  Γ ⊢i (a ---> p ---> b ---> c) using i ->
+  Γ ⊢i (a ---> q ---> b ---> c) using i->
+  Γ ⊢i (a ---> (p or q) ---> b ---> c) using i.
+Proof.
+  intros WFa WFb WFp WFq WFc H H0.
+  toMLGoal.
+  { wf_auto2. } 
+  repeat mlIntro.
+  mlDestructOr 1.
+  - fromMLGoal. apply H.
+  - fromMLGoal. apply H0.
+Defined.
+
+Lemma pf_iff_split {Σ : Signature} Γ A B i:
+  well_formed A ->
+  well_formed B ->
+  Γ ⊢i A ---> B using i ->
+  Γ ⊢i B ---> A using i ->
+  Γ ⊢i A <---> B using i.
+Proof.
+  intros wfA wfB AimplB BimplA.
+  unfold patt_iff.
+  apply conj_intro_meta; try_wfauto2; assumption.
+Defined.
+
+Lemma pf_iff_proj1 {Σ : Signature} Γ A B i:
+  well_formed A ->
+  well_formed B ->
+  Γ ⊢i A <---> B using i ->
+  Γ ⊢i A ---> B using i.
+Proof.
+  intros WFA WFB H. unfold patt_iff in H.
+  apply pf_conj_elim_l_meta in H; try_wfauto2; assumption.
+Defined.
+
+Lemma pf_iff_proj2 {Σ : Signature} Γ A B i:
+  well_formed A ->
+  well_formed B ->
+  Γ ⊢i (A <---> B) using i ->
+  Γ ⊢i (B ---> A) using i.
+Proof.
+  intros WFA WFB H. unfold patt_iff in H.
+  apply pf_conj_elim_r_meta in H; try_wfauto2; assumption.
+Defined.
+
+Lemma pf_iff_iff {Σ : Signature} Γ A B i:
+  well_formed A ->
+  well_formed B ->
+  prod ((Γ ⊢i (A <---> B) using i) -> (prod (Γ ⊢i (A ---> B) using i) (Γ ⊢i (B ---> A) using i)))
+  ( (prod (Γ ⊢i (A ---> B) using i)  (Γ ⊢i (B ---> A) using i)) -> (Γ ⊢i (A <---> B) using i)).
+Proof.
+  intros WFA WFB.
+  split; intros H.
+  {
+    pose proof (H1 := pf_iff_proj1 WFA WFB H).
+    pose proof (H2 := pf_iff_proj2 WFA WFB H).
+    split; assumption.
+  }
+  {
+    destruct H as [H1 H2].
+    apply pf_iff_split; assumption.
+  }
+Defined.
+
+Lemma pf_iff_equiv_refl {Σ : Signature} Γ A :
+  well_formed A ->
+  Γ ⊢i (A <---> A) using BasicReasoning.
+Proof.
+  intros WFA.
+  apply pf_iff_split; try_wfauto2; apply A_impl_A; assumption.
+Defined.
+
+Lemma pf_iff_equiv_sym {Σ : Signature} Γ A B i:
+  well_formed A ->
+  well_formed B ->
+  Γ ⊢i (A <---> B) using i ->
+  Γ ⊢i (B <---> A) using i.
+Proof.
+  intros wfA wfB H.
+  pose proof (H2 := H).
+  apply pf_iff_proj2 in H2; try_wfauto2.
+  rename H into H1.
+  apply pf_iff_proj1 in H1; try_wfauto2.
+  apply pf_iff_split; try_wfauto2; assumption.
+Defined.
+
+Lemma pf_iff_equiv_trans {Σ : Signature} Γ A B C i:
+  well_formed A ->
+  well_formed B ->
+  well_formed C ->
+  Γ ⊢i (A <---> B) using i ->
+  Γ ⊢i (B <---> C) using i ->
+  Γ ⊢i (A <---> C) using i.
+Proof.
+  intros wfA wfB wfC AeqB BeqC.
+  apply pf_iff_iff in AeqB; try_wfauto2. destruct AeqB as [AimpB BimpA].
+  apply pf_iff_iff in BeqC; try_wfauto2. destruct BeqC as [BimpC CimpB].
+  apply pf_iff_iff; try_wfauto2.
+  split.
+  {
+    eapply syllogism_meta. 4,5: eassumption.
+    1-3: wf_auto2.
+  }
+  {
+    eapply syllogism_meta. 4,5: eassumption.
+    1-3: wf_auto2.
+  }
+Defined.
+
+Lemma prf_conclusion {Σ : Signature} Γ a b i:
+  well_formed a ->
+  well_formed b ->
+  Γ ⊢i b using i ->
+  Γ ⊢i (a ---> b) using i.
+Proof.
+  intros WFa WFb H. eapply MP.
+  apply H.
+  useBasicReasoning.
+  apply P1; wf_auto2.
+Defined.
+
+
+
+Lemma and_of_negated_iff_not_impl {Σ : Signature} Γ p1 p2:
+well_formed p1 ->
+well_formed p2 ->
+Γ ⊢i (! (! p1 ---> p2) <---> ! p1 and ! p2)
+using BasicReasoning.
+Proof.
+intros wfp1 wfp2.
+apply conj_intro_meta.
+{ wf_auto2. }
+{ wf_auto2. }
+- toMLGoal.
+  { wf_auto2. }
+  mlIntro. mlIntro.
+  mlApply 0.
+  mlIntro.
+  unfold patt_or.
+  mlAdd (@not_not_elim Σ Γ p2 ltac:(wf_auto2)).
+  mlApply 0.
+  mlApply 2.
+  mlAdd (@not_not_intro Σ Γ (! p1) ltac:(wf_auto2)).
+  mlApply 0.
+  mlExactn 4.
+- toMLGoal.
+  { wf_auto2. }
+  mlIntro. mlIntro.
+  unfold patt_and.
+  mlApply 0.
+  unfold patt_or.
+  mlIntro.
+  mlAdd (@not_not_intro Σ Γ p2 ltac:(wf_auto2)).
+  mlApply 0.
+  mlApply 2.
+  mlAdd (@not_not_elim Σ Γ (! p1) ltac:(wf_auto2)).
+  mlApply 0.
+  mlExactn 4.
+Defined.
+
+Lemma and_impl_2 {Σ : Signature} Γ p1 p2:
+well_formed p1 ->
+well_formed p2 ->
+Γ ⊢i (! (p1 ---> p2) <---> p1 and ! p2)
+using BasicReasoning.
+Proof.
+intros wfp1 wfp2.
+apply conj_intro_meta.
+{ wf_auto2. }
+{ wf_auto2. }
+- toMLGoal.
+  { wf_auto2. }
+  mlIntro. mlIntro.
+  mlApply 0.
+  mlIntro.
+  unfold patt_or.
+  mlAdd (@not_not_elim Σ Γ p2 ltac:(wf_auto2)).
+  mlApply 0.
+  mlApply 2.
+  mlAdd (@not_not_intro Σ Γ p1 ltac:(wf_auto2)).
+  mlApply 0.
+  mlExactn 4.
+- toMLGoal.
+  { wf_auto2. }
+  mlIntro. mlIntro.
+  mlApply 0.
+  unfold patt_or.
+  mlIntro.
+  mlAdd (@not_not_intro Σ Γ p2 ltac:(wf_auto2)).
+  mlApply 0.
+  mlApply 2.
+  mlAdd (@not_not_elim Σ Γ p1 ltac:(wf_auto2)).
+  mlApply 0.
+  mlExactn 4.
+Defined.
+
+Lemma conj_intro_meta_partial {Σ : Signature} (Γ : Theory) (A B : Pattern) (i : ProofInfo) :
+well_formed A → well_formed B →
+Γ ⊢i A using i →
+Γ ⊢i B ---> (A and B) using i.
+Proof.
+intros WFA WFB H.
+eapply MP.
+- exact H.
+- useBasicReasoning. apply conj_intro.
+  { wf_auto2. }
+  { wf_auto2. }
+Defined.
+
+Lemma and_impl_patt {Σ : Signature} (A B C : Pattern) Γ (i : ProofInfo):
+well_formed A → well_formed B → well_formed C →
+Γ ⊢i A using i ->
+Γ ⊢i ((A and B) ---> C) using i ->
+Γ ⊢i (B ---> C) using i.
+Proof.
+intros WFA WFB WFC H H0.
+eapply syllogism_meta with (B := patt_and A B).
+{ wf_auto2. }
+{ wf_auto2. }
+{ wf_auto2. }
+2: { exact H0. }
+apply conj_intro_meta_partial.
+{ wf_auto2. }
+{ wf_auto2. }
+exact H.
+Defined.
+
+Lemma conj_intro2 {Σ : Signature} (Γ : Theory) (A B : Pattern) :
+well_formed A -> well_formed B ->
+Γ ⊢i (A ---> (B ---> (B and A)))
+using BasicReasoning.
+Proof.
+intros WFA WFB. eapply reorder_meta.
+{ wf_auto2. }
+{ wf_auto2. }
+{ wf_auto2. }
+apply conj_intro.
+{ wf_auto2. }
+{ wf_auto2. }
+Defined.
+
+Lemma conj_intro_meta_partial2  {Σ : Signature} (Γ : Theory) (A B : Pattern) (i : ProofInfo):
+well_formed A → well_formed B →
+Γ ⊢i A using i →
+Γ ⊢i B ---> (B and A) using i.
+Proof.
+intros WFA WFB H.
+eapply MP.
+- exact H.
+- useBasicReasoning. apply conj_intro2.
+  { wf_auto2. }
+  { wf_auto2. }
+Defined.
+
+Lemma and_impl_patt2 {Σ : Signature}  (A B C : Pattern) Γ (i : ProofInfo):
+well_formed A → well_formed B → well_formed C →
+Γ ⊢i A using i ->
+Γ ⊢i ((B and A) ---> C) using i ->
+Γ ⊢i (B ---> C) using i.
+Proof.
+intros WFA WFB WFC H H0.
+eapply syllogism_meta with (B := patt_and B A).
+{ wf_auto2. }
+{ wf_auto2. }
+{ wf_auto2. }
+2: exact H0.
+apply conj_intro_meta_partial2.
+{ wf_auto2. }
+{ wf_auto2. }
+exact H.
+Defined.
+
+
+Lemma patt_and_comm_meta {Σ : Signature} (A B : Pattern) (Γ : Theory) (i : ProofInfo) :
+well_formed A → well_formed B
+->
+Γ ⊢i A and B using i ->
+Γ ⊢i B and A using i.
+Proof.
+intros WFA WFB H.
+apply pf_conj_elim_r_meta in H as P1.
+apply pf_conj_elim_l_meta in H as P2. all: try_wfauto2.
+apply conj_intro_meta; assumption.
+Defined.
+
+Lemma MLGoal_applyMeta {Σ : Signature} Γ r r' i:
+Γ ⊢i (r' ---> r) using i ->
+forall l,
+@mkMLGoal Σ Γ l r' i ->
+@mkMLGoal Σ Γ l r i.
+Proof.
+intros Himp l H.
+unfold of_MLGoal in *. simpl in *.
+intros wfr wfl.
+eapply prf_weaken_conclusion_iter_meta_meta.
+4: apply Himp.
+4: apply H.
+all: try assumption.
+1,2: pose proof (wfrr' := proved_impl_wf _ _ (proj1_sig Himp)); wf_auto2.
+Defined.
+
+
+
+
+
+Tactic Notation "mlApplyMeta" uconstr(t) :=
+  eapply (@MLGoal_applyMeta _ _ _ _ _ t).
+
+Lemma MLGoal_left {Σ : Signature} Γ l x y i:
+  @mkMLGoal Σ Γ l x i ->
+  @mkMLGoal Σ Γ l (patt_or x y) i.
+Proof.
+  intros H.
+  unfold of_MLGoal in *. simpl in *.
+  intros wfxy wfl.
+  eapply prf_weaken_conclusion_iter_meta_meta.
+  4: { useBasicReasoning. apply disj_left_intro. wf_auto2. wf_auto2. }
+  { wf_auto2. }
+  { wf_auto2. }
+  { wf_auto2. }
+  apply H.
+  { wf_auto2. }
+  { assumption. }
+Defined.
+
+Lemma MLGoal_right {Σ : Signature} Γ l x y i:
+  @mkMLGoal Σ Γ l y i ->
+  @mkMLGoal Σ Γ l (patt_or x y) i.
+Proof.
+  intros H.
+  unfold of_MLGoal in *. simpl in *.
+  intros wfxy wfl.
+  eapply prf_weaken_conclusion_iter_meta_meta.
+  4: { useBasicReasoning. apply disj_right_intro. wf_auto2. wf_auto2. }
+  { wf_auto2. }
+  { wf_auto2. }
+  { wf_auto2. }
+  apply H.
+  { wf_auto2. }
+  { assumption. }
+Defined.
+
+Ltac mlLeft := apply MLGoal_left.
+Ltac mlRight := apply MLGoal_right.
+
+Example ex_mlLeft {Σ : Signature} Γ a:
+  well_formed a ->
+  Γ ⊢i a ---> (a or a)
+  using BasicReasoning.
+Proof.
+  intros wfa.
+  toMLGoal.
+  { wf_auto2. }
+  mlIntro.
+  mlLeft.
+Abort.
+
+Lemma MLGoal_applyMetaIn {Σ : Signature} Γ r r' i:
+  Γ ⊢i (r ---> r') using i ->
+  forall l₁ l₂ g,
+    @mkMLGoal Σ Γ (l₁ ++ r'::l₂) g i ->
+    @mkMLGoal Σ Γ (l₁ ++ r::l₂ ) g i.
+Proof.
+  intros Himp l₁ l₂ g H.
+  unfold of_MLGoal in *. simpl in *.
+  intros wfg Hwf.
+  specialize (H wfg).
+  eapply prf_strenghten_premise_iter_meta_meta.
+  6: apply Himp.
+  6: apply H.
+  { abstract (apply wfapp_proj_1 in Hwf; exact Hwf). }
+  { abstract (apply wfl₁hl₂_proj_l₂ in Hwf; exact Hwf). }
+  { abstract (pose proof (Himp' := proj1_sig Himp); apply proved_impl_wf in Himp'; wf_auto2). }
+  { abstract (apply wfl₁hl₂_proj_h in Hwf; exact Hwf). }
+  { exact wfg. }
+  { abstract(
+      pose proof (wfapp_proj_1 Hwf);
+      pose proof (wfl₁hl₂_proj_l₂ Hwf);
+      pose proof (wfl₁hl₂_proj_h Hwf);
+      unfold Pattern.wf;
+      rewrite map_app;
+      rewrite foldr_app;
+      simpl;
+      pose proof (Himp' := proj1_sig Himp);
+      apply proved_impl_wf in Himp';
+      apply well_formed_imp_proj2 in Himp';
+      rewrite Himp';
+      simpl;
+      unfold Pattern.wf in H1;
+      rewrite H1;
+      exact H0
+    ).
+ }
+Defined.
+
+Tactic Notation "mlApplyMeta" uconstr(t) "in" constr(n) :=
+  eapply cast_proof_ml_hyps;
+  [(let hyps := fresh "hyps" in
+    rewrite <- (firstn_skipn n);
+    rewrite [hyps in (hyps ++ _)]/=;
+    rewrite [hyps in (_ ++ hyps)]/=;
+    reflexivity
+   )|];
+  eapply (@MLGoal_applyMetaIn _ _ _ _ _ t);
+  eapply cast_proof_ml_hyps;
+  [(rewrite /app; reflexivity)|].
+
+Local Example Private_ex_mlApplyMetaIn {Σ : Signature} Γ p q:
+  well_formed p ->
+  well_formed q ->
+  Γ ⊢i p ---> (p or q)
+  using BasicReasoning.
+Proof.
+  intros wfp wfq.
+  toMLGoal.
+  { wf_auto2. }
+  mlIntro.
+  mlApplyMeta (@disj_left_intro Σ Γ p q ltac:(wf_auto2) ltac:(wf_auto2)) in 0.
+  mlExactn 0.
+Defined.
+
+Lemma MLGoal_destructAnd {Σ : Signature} Γ g l₁ l₂ x y i:
+    @mkMLGoal Σ Γ (l₁ ++ x::y::l₂ ) g i ->
+    @mkMLGoal Σ Γ (l₁ ++ (x and y)::l₂) g i .
+Proof.
+  intros H.
+  unfold of_MLGoal. intros wfg Hwf. pose proof (wfg' := wfg). pose proof (Hwf' := Hwf).
+  revert wfg' Hwf'.
+  cut (of_MLGoal (@mkMLGoal Σ Γ (l₁ ++ (x and y)::l₂ ) g i)).
+  { auto. }
+  simpl in wfg, Hwf.
+
+  mlAssert (y) using first (length (l₁ ++ [x and y])).
+  { abstract (
+      apply wfapp_proj_2 in Hwf;
+      unfold Pattern.wf in Hwf;
+      simpl in Hwf;
+      apply andb_prop in Hwf;
+      destruct Hwf as [wfxy _];
+      wf_auto2
+    ).
+  }
+  {
+    eapply cast_proof_ml_hyps.
+    { replace (l₁ ++ (x and y) :: l₂) with ((l₁++ [x and y]) ++ l₂).
+      2: { rewrite -app_assoc. reflexivity. }
+      rewrite take_app.
+      reflexivity.
+    }
+    assert (well_formed x).
+    {
+      abstract (
+        apply wfapp_proj_2 in Hwf;
+        unfold Pattern.wf in Hwf;
+        simpl in Hwf;
+        apply andb_prop in Hwf as [wfxy _];
+        wf_auto2
+      ).
+    }
+    useBasicReasoning.
+    mlApplyMeta (@pf_conj_elim_r Σ Γ x y ltac:(assumption) ltac:(assumption)).
+    apply MLGoal_exactn.
+  }
+
+  eapply cast_proof_ml_hyps.
+  {  
+    replace (l₁ ++ (x and y) :: l₂) with ((l₁++ [x and y]) ++ l₂).
+    2: { rewrite -app_assoc. reflexivity. }
+    rewrite take_app. rewrite drop_app. reflexivity.
+  }
+
+  mlAssert (x) using first (length (l₁ ++ [x and y])).
+  { abstract (
+      apply wfapp_proj_2 in Hwf;
+      unfold Pattern.wf in Hwf;
+      simpl in Hwf;
+      apply andb_prop in Hwf;
+      destruct Hwf as [wfxy _];
+      wf_auto2
+    ).
+  }
+  {
+    eapply cast_proof_ml_hyps.
+    {
+      replace (l₁ ++ (x and y) :: l₂) with ((l₁++ [x and y]) ++ l₂).
+      2: { rewrite -app_assoc. reflexivity. }
+      rewrite take_app.
+      reflexivity.
+    }
+    assert (well_formed x).
+    {
+      abstract (
+        apply wfapp_proj_2 in Hwf;
+        unfold Pattern.wf in Hwf;
+        simpl in Hwf;
+        apply andb_prop in Hwf as [wfxy _];
+        wf_auto2
+      ).
+    }
+    useBasicReasoning.
+    mlApplyMeta (@pf_conj_elim_l Σ Γ x y ltac:(assumption) ltac:(assumption)).
+    apply MLGoal_exactn.
+  }
+
+  eapply cast_proof_ml_hyps.
+  {  
+    replace (l₁ ++ (x and y) :: l₂) with ((l₁++ [x and y]) ++ l₂).
+    2: { rewrite -app_assoc. reflexivity. }
+    rewrite take_app. rewrite drop_app. reflexivity.
+  }
+
+  eapply cast_proof_ml_hyps.
+  {
+    rewrite -app_assoc. reflexivity.
+  }
+
+ apply myGoal_clear_hyp.  
+ exact H.
+Defined.
+
+Tactic Notation "mlDestructAnd" constr(n) :=
+  eapply cast_proof_ml_hyps;
+  [(let hyps := fresh "hyps" in
+    rewrite <- (firstn_skipn n);
+    rewrite [hyps in (hyps ++ _)]/=;
+    rewrite [hyps in (_ ++ hyps)]/=;
+    reflexivity
+   )|];
+  apply MLGoal_destructAnd;
+  eapply cast_proof_ml_hyps;
+  [(rewrite /app; reflexivity)|].
+
+Local Example ex_mlDestructAnd {Σ : Signature} Γ a b p q:
+  well_formed a ->
+  well_formed b ->
+  well_formed p ->
+  well_formed q ->
+  Γ ⊢i p and q ---> a and b ---> q ---> a
+  using BasicReasoning.
+Proof.
+  intros. toMLGoal.
+  { wf_auto2. }
+  do 3 mlIntro.
+  mlDestructAnd 1.
+  mlDestructAnd 0.
+  mlExactn 2.
+Defined.
+
+ 
+Lemma and_of_equiv_is_equiv {Σ : Signature} Γ p q p' q' i:
+well_formed p ->
+well_formed q ->
+well_formed p' ->
+well_formed q' ->
+Γ ⊢i (p <---> p') using i ->
+Γ ⊢i (q <---> q') using i ->
+Γ ⊢i ((p and q) <---> (p' and q')) using i.
+Proof.
+intros wfp wfq wfp' wfq' pep' qeq'.
+pose proof (pip' := pep'). apply pf_conj_elim_l_meta in pip'; auto.
+pose proof (p'ip := pep'). apply pf_conj_elim_r_meta in p'ip; auto.
+pose proof (qiq' := qeq'). apply pf_conj_elim_l_meta in qiq'; auto.
+pose proof (q'iq := qeq'). apply pf_conj_elim_r_meta in q'iq; auto.
+
+apply conj_intro_meta; auto.
+- toMLGoal.
+  { wf_auto2. }
+  mlIntro. unfold patt_and.
+  mlIntro. mlApply 0.
+  mlDestructOr 1.
+  + apply modus_tollens in pip'; auto 10.
+    mlAdd pip'.
+    mlLeft.
+    mlApply 0.
+    mlExactn 2.
+  + apply modus_tollens in qiq'; auto 10.
+    mlAdd qiq'.
+    mlRight.
+    mlApply 0.
+    mlExactn 2.
+- toMLGoal.
+  { wf_auto2. }
+  mlIntro. unfold patt_and.
+  mlIntro. mlApply 0.
+  mlDestructOr 1.
+  + mlLeft.
+    apply modus_tollens in p'ip; auto.
+    mlAdd p'ip.
+    mlApply 0.
+    mlExactn 2.
+  + mlRight.
+    apply modus_tollens in q'iq; auto.
+    mlAdd q'iq.
+    mlApply 0.
+    mlExactn 2.
+Defined. 
+
+Lemma or_of_equiv_is_equiv {Σ : Signature} Γ p q p' q' i:
+well_formed p ->
+well_formed q ->
+well_formed p' ->
+well_formed q' ->
+Γ ⊢i (p <---> p') using i ->
+Γ ⊢i (q <---> q') using i ->
+Γ ⊢i ((p or q) <---> (p' or q')) using i.
+Proof with try_wfauto2.
+intros wfp wfq wfp' wfq' pep' qeq'.
+pose proof (pip' := pep'). apply pf_conj_elim_l_meta in pip'...
+pose proof (p'ip := pep'). apply pf_conj_elim_r_meta in p'ip...
+pose proof (qiq' := qeq'). apply pf_conj_elim_l_meta in qiq'...
+pose proof (q'iq := qeq'). apply pf_conj_elim_r_meta in q'iq...
+
+apply conj_intro_meta; auto.
+- toMLGoal.
+  { auto. }
+  mlIntro.
+  mlDestructOr 0.
+  + mlLeft. fromMLGoal. assumption.
+  + mlRight. fromMLGoal. assumption.
+- toMLGoal.
+  { auto. }
+  mlIntro.
+  mlDestructOr 0.
+  + mlLeft. fromMLGoal. assumption.
+  + mlRight. fromMLGoal. assumption.
+Defined.
+
+
+Lemma impl_iff_notp_or_q {Σ : Signature} Γ p q:
+well_formed p ->
+well_formed q ->
+Γ ⊢i ((p ---> q) <---> (! p or q))
+using BasicReasoning.
+Proof.
+intros wfp wfq.
+apply conj_intro_meta; auto.
+- toMLGoal.
+  { wf_auto2. }
+  mlIntro.
+  mlAdd (@A_or_notA Σ Γ p wfp).
+  mlDestructOr 0.
+  + mlRight.
+    mlApply 1.
+    mlExactn 0.
+  + mlLeft.
+    mlExactn 0.
+- toMLGoal.
+  { wf_auto2. }
+  mlIntro. mlIntro. unfold patt_or.
+  mlApply 0.
+  mlApplyMeta (@not_not_intro _ _ p wfp).
+  mlExactn 1.
+Defined.
+
+Lemma p_and_notp_is_bot {Σ : Signature} Γ p:
+well_formed p ->
+Γ ⊢i (⊥ <---> p and ! p)
+using BasicReasoning.
+Proof.
+intros wfp.
+apply conj_intro_meta; auto.
+- apply bot_elim; auto.
+- unfold patt_and.
+  toMLGoal.
+  { wf_auto2. }
+  mlIntro.
+  mlApply 0.
+  mlAdd (@A_or_notA Σ Γ (! p) ltac:(wf_auto2)).
+  mlExactn 0.
+Defined.
+
+Lemma weird_lemma  {Σ : Signature} Γ A B L R:
+well_formed A ->
+well_formed B ->
+well_formed L ->
+well_formed R ->
+Γ ⊢i (((L and A) ---> (B or R)) ---> (L ---> ((A ---> B) or R)))
+using BasicReasoning.
+Proof.
+intros wfA wfB wfL wfR.
+toMLGoal.
+{ wf_auto2. }
+mlIntro. mlIntro.
+mlAdd (@A_or_notA Σ Γ A wfA).
+mlDestructOr 0.
+- mlAssert ((B or R)).
+  { wf_auto2. }
+  { mlApply 1.
+    unfold patt_and at 2.
+    mlIntro.
+    mlDestructOr 3.
+    + mlApply 3. mlExactn 2.
+    + mlApply 3. mlExactn 0.
+  }
+  mlDestructOr 3.
+  + mlLeft. mlIntro. mlExactn 3.
+  + mlRight. mlExactn 3.
+- mlLeft.
+  mlIntro.
+  mlApplyMeta (@bot_elim Σ _ B wfB).
+  mlApply 0. mlExactn 3.
+Defined.
+
+Lemma weird_lemma_meta {Σ : Signature} Γ A B L R i:
+well_formed A ->
+well_formed B ->
+well_formed L ->
+well_formed R ->
+Γ ⊢i ((L and A) ---> (B or R)) using i ->
+Γ ⊢i (L ---> ((A ---> B) or R)) using i.
+Proof.
+intros WFA WFB WFL WFR H.
+eapply MP.
+2: { useBasicReasoning. apply weird_lemma; assumption. }
+exact H.
+Defined.
+
+Lemma imp_trans_mixed_meta {Σ : Signature} Γ A B C D i :
+well_formed A -> well_formed B -> well_formed C -> well_formed D ->
+Γ ⊢i (C ---> A) using i ->
+Γ ⊢i (B ---> D) using i ->
+Γ ⊢i ((A ---> B) ---> C ---> D) using i.
+Proof.
+intros WFA WFB WFC WFD H H0.
+epose proof (H1 := @prf_weaken_conclusion Σ Γ A B D WFA WFB WFD).
+eapply useBasicReasoning in H1.
+eapply MP in H1.
+2: { exact H0. }
+epose proof (H2 := @prf_strenghten_premise Σ Γ A C D WFA WFC WFD).
+eapply useBasicReasoning in H2.
+eapply MP in H2.
+2: { exact H. }
+epose proof (H3 := @syllogism_meta Σ Γ _ _ _ i _ _ _ H1 H2).
+exact H3.
+Unshelve. all: wf_auto2.
+Defined.
+
+Lemma and_weaken {Σ : Signature} A B C Γ i:
+well_formed A -> well_formed B -> well_formed C ->
+Γ ⊢i (B ---> C) using i ->
+Γ ⊢i ((A and B) ---> (A and C)) using i.
+Proof.
+intros WFA WFB WFC H.
+epose proof (H0 := @and_impl' Σ Γ A B (A and C) _ _ _).
+eapply MP. 2: { useBasicReasoning. exact H0. }
+apply reorder_meta.
+1-3: wf_auto2.
+epose proof (H1 := @prf_strenghten_premise Σ Γ C B (A ---> A and C) _ _ _).
+eapply MP.
+2: eapply MP.
+3: { useBasicReasoning. exact H1. }
+2: { exact H. }
+useBasicReasoning.
+apply conj_intro2; assumption.
+Unshelve.
+all: wf_auto2.
+Defined.
+
+Lemma impl_and {Σ : Signature} Γ A B C D i: 
+well_formed A -> well_formed B -> well_formed C -> well_formed D ->
+Γ ⊢i (A ---> B) using i ->
+Γ ⊢i (C ---> D) using i ->
+Γ ⊢i (A and C) ---> (B and D) using i.
+Proof.
+intros WFA WFB WFC WFD H H0.
+toMLGoal.
+{ wf_auto2. }
+{
+  mlAdd H.
+  mlAdd H0.
+  mlIntro.
+  mlDestructAnd 2.
+  mlIntro.
+  mlDestructOr 4.
+  {
+    mlApply 4.
+    mlApply 1.
+    mlExactn 2.
+  }
+  {
+    mlApply 4.
+    mlApply 0.
+    mlExactn 3.
+  }
+}
+Defined.
+
+Lemma and_drop {Σ : Signature} A B C Γ i:
+well_formed A -> well_formed B -> well_formed C ->
+Γ ⊢i ((A and B) ---> C) using i ->
+Γ ⊢i ((A and B) ---> (A and C)) using i.
+Proof.
+intros WFA WFB WFC H.
+toMLGoal.
+{ wf_auto2. }
+mlAdd H.
+mlIntro.
+mlIntro.
+mlDestructOr 2.
+{
+  mlDestructAnd 1.
+  mlApply 3.
+  mlExactn 1.
+}
+{
+  mlApply 2.
+  mlApply 0.
+  mlExactn 1.
+}
+Defined.
+
+
+Lemma prf_equiv_of_impl_of_equiv {Σ : Signature} Γ a b a' b' i:
+well_formed a = true ->
+well_formed b = true ->
+well_formed a' = true ->
+well_formed b' = true ->
+Γ ⊢i (a <---> a') using i ->
+Γ ⊢i (b <---> b') using i ->
+Γ ⊢i (a ---> b) <---> (a' ---> b') using i
+.
+Proof.
+intros wfa wfb wfa' wfb' Haa' Hbb'.
+unshelve(epose proof (Haa'1 := @pf_conj_elim_l_meta _ _ _ _ _ _ _ Haa')).
+{ wf_auto2. }
+{ wf_auto2. }
+unshelve(epose proof (Haa'2 := @pf_conj_elim_r_meta _ _ _ _ _ _ _ Haa')).
+{ wf_auto2. }
+{ wf_auto2. }
+unshelve(epose proof (Hbb'1 := @pf_conj_elim_l_meta _ _ _ _ _ _ _ Hbb')).
+{ wf_auto2. }
+{ wf_auto2. }
+unshelve(epose proof (Hbb'2 := @pf_conj_elim_r_meta _ _ _ _ _ _ _ Hbb')).
+{ wf_auto2. }
+{ wf_auto2. }
+
+apply pf_iff_equiv_trans with (B := (a ---> b')).
+1-3: wf_auto2.
+  + apply conj_intro_meta.
+    1-2: wf_auto2.
+    * toMLGoal.
+      { wf_auto2. }
+      mlIntro. mlIntro.
+      mlAdd Hbb'1.
+      mlApply 0.
+      mlApply 1.
+      mlExactn 2.
+    * toMLGoal.
+      { wf_auto2. }
+      mlIntro. mlIntro.
+      mlAdd Hbb'2.
+      mlApply 0.
+      mlApply 1.
+      mlExactn 2.
+  + apply conj_intro_meta.
+    1-2: wf_auto2.
+    * toMLGoal.
+      { wf_auto2. }
+      mlIntro. mlIntro.
+      mlAdd Haa'2.
+      mlApply 1.
+      mlApply 0.
+      mlExactn 2.
+    * toMLGoal.
+      { wf_auto2. }
+      mlIntro. mlIntro.
+      mlAdd Haa'1.
+      mlApply 1.
+      mlApply 0.
+      mlExactn 2.
+Defined.
+
+
+
+Lemma lhs_to_and {Σ : Signature} Γ a b c i:
+  well_formed a ->
+  well_formed b ->
+  well_formed c ->
+  Γ ⊢i (a and b) ---> c using i ->
+  Γ ⊢i a ---> b ---> c using i.
+Proof.
+  intros wfa wfb wfc H.
+  toMLGoal.
+  { wf_auto2. }
+  do 2 mlIntro. mlApplyMeta H.
+  fromMLGoal.
+  useBasicReasoning.
+  apply conj_intro.
+  { wf_auto2. }
+  { wf_auto2. }
+Defined.
+
+Lemma lhs_from_and {Σ : Signature} Γ a b c i:
+  well_formed a ->
+  well_formed b ->
+  well_formed c ->
+  Γ ⊢i a ---> b ---> c using i ->
+  Γ ⊢i (a and b) ---> c using i.
+Proof.
+  intros wfa wfb wfc H.
+  toMLGoal.
+  { wf_auto2. }
+  mlIntro.
+  mlAssert (b).
+  { wf_auto2. }
+  { fromMLGoal. useBasicReasoning. apply pf_conj_elim_r.
+    wf_auto2. wf_auto2.
+  }
+  mlAssert (a) using first 1.
+  { wf_auto2. }
+  { fromMLGoal. useBasicReasoning. apply pf_conj_elim_l; wf_auto2. }
+  mlAdd H.
+  mlAssert ((b ---> c)).
+  { wf_auto2. }
+  { mlApply 0. mlExactn 2. }
+  mlApply 4.
+  mlExactn 3.
+Defined.
+
+Lemma prf_conj_split {Σ : Signature} Γ a b l:
+  well_formed a ->
+  well_formed b ->
+  Pattern.wf l ->
+  Γ ⊢i (foldr patt_imp a l) ---> (foldr patt_imp b l) ---> (foldr patt_imp (a and b) l)
+  using BasicReasoning.
+Proof.
+  intros wfa wfb wfl.
+  induction l.
+  - simpl. apply conj_intro; assumption.
+  - simpl. pose proof (wfl' := wfl). unfold Pattern.wf in wfl'. simpl in wfl'. apply andb_prop in wfl' as [wfa0 wfl'].
+    specialize (IHl wfl').
+    toMLGoal.
+    { wf_auto2. }
+    do 3 mlIntro.
+    mlAssert ((foldr patt_imp a l)).
+    { wf_auto2. }
+    { mlApply 0. mlExactn 2. }
+    mlAssert ((foldr patt_imp b l)).
+    { wf_auto2. }
+    { mlApply 1. mlExactn 2. }
+    mlClear 2. mlClear 1. mlClear 0.
+    fromMLGoal. apply IHl.
+Defined.
+
+Lemma prf_conj_split_meta {Σ : Signature} Γ a b l (i : ProofInfo):
+  well_formed a ->
+  well_formed b ->
+  Pattern.wf l ->
+  Γ ⊢i (foldr patt_imp a l) using i -> 
+  Γ ⊢i (foldr patt_imp b l) ---> (foldr patt_imp (a and b) l) using i.
+Proof.
+  intros. eapply MP. 2: { useBasicReasoning. apply prf_conj_split; assumption. }
+  exact H2.
+Defined.
+
+Lemma prf_conj_split_meta_meta {Σ : Signature} Γ a b l (i : ProofInfo):
+  well_formed a ->
+  well_formed b ->
+  Pattern.wf l ->
+  Γ ⊢i (foldr patt_imp a l) using i -> 
+  Γ ⊢i (foldr patt_imp b l) using i ->
+  Γ ⊢i (foldr patt_imp (a and b) l) using i.
+Proof.
+  intros. eapply MP.
+  2: {
+    apply prf_conj_split_meta; assumption.
+  }
+  exact H3.
+Defined.
+
+Lemma MLGoal_splitAnd {Σ : Signature} Γ a b l i:
+  @mkMLGoal Σ Γ l a i ->
+  @mkMLGoal Σ Γ l b i ->
+  @mkMLGoal Σ Γ l (a and b) i.
+Proof.
+  intros Ha Hb.
+  unfold of_MLGoal in *. simpl in *.
+  intros wfab wfl.
+  feed specialize Ha.
+  { abstract(wf_auto2). }
+  { exact wfl. }
+  feed specialize Hb.
+  { abstract(wf_auto2). }
+  { exact wfl. }
+  apply prf_conj_split_meta_meta; auto.
+  { abstract (wf_auto2). }
+  { abstract (wf_auto2). }
+Defined.
+
+Ltac mlSplitAnd := apply MLGoal_splitAnd.
+
+Local Lemma ex_mlSplitAnd {Σ : Signature} Γ a b c:
+  well_formed a ->
+  well_formed b ->
+  well_formed c ->
+  Γ ⊢i a ---> b ---> c ---> (a and b)
+  using BasicReasoning.
+Proof.
+  intros wfa wfb wfc.
+  toMLGoal.
+  { wf_auto2. }
+  mlIntro. mlIntro. mlIntro.
+  mlSplitAnd.
+  - mlExactn 0.
+  - mlExactn 1.
+Defined.
+
+Lemma prf_local_goals_equiv_impl_full_equiv {Σ : Signature} Γ g₁ g₂ l:
+  well_formed g₁ ->
+  well_formed g₂ ->
+  Pattern.wf l ->
+  Γ ⊢i (foldr patt_imp (g₁ <---> g₂) l) --->
+      ((foldr patt_imp g₁ l) <---> (foldr patt_imp g₂ l))
+  using BasicReasoning.
+Proof.
+  intros wfg₁ wfg₂ wfl.
+  induction l; simpl.
+  - apply A_impl_A; wf_auto2.
+  - pose proof (wfl' := wfl). unfold Pattern.wf in wfl'. simpl in wfl'. apply andb_prop in wfl' as [wfa wfl'].
+    specialize (IHl wfl').
+    toMLGoal.
+    { wf_auto2. }
+    mlIntro. mlSplitAnd.
+    + unshelve (mlApplyMeta (@P2 _ _ _ _ _ _ _ _)).
+      1-3: wf_auto2.
+      (* TODO we need some [mlRevert] tactic *)
+      fromMLGoal. toMLGoal.
+      { wf_auto2. }
+      unshelve(mlApplyMeta (@P2 _ _ _ _ _ _ _ _)).
+      1-3: wf_auto2.
+      mlIntro. mlClear 0. mlIntro.
+      mlApplyMeta IHl in 0. unfold patt_iff at 1. mlDestructAnd 0.
+      mlExactn 0.
+    + unshelve (mlApplyMeta (@P2 _ _ _ _ _ _ _ _)).
+      1-3: wf_auto2.
+      fromMLGoal. toMLGoal.
+      { wf_auto2. }
+      unshelve (mlApplyMeta (@P2 _ _ _ _ _ _ _ _)).
+      1-3: wf_auto2.
+      mlIntro. mlClear 0. mlIntro.
+      mlApplyMeta IHl in 0. unfold patt_iff at 1. mlDestructAnd 0.
+      mlExactn 1.
+Defined.
+
+Lemma prf_local_goals_equiv_impl_full_equiv_meta {Σ : Signature} Γ g₁ g₂ l i:
+  well_formed g₁ ->
+  well_formed g₂ ->
+  Pattern.wf l ->
+  Γ ⊢i (foldr patt_imp (g₁ <---> g₂) l) using i ->
+  Γ ⊢i ((foldr patt_imp g₁ l) <---> (foldr patt_imp g₂ l)) using i.
+Proof.
+  intros wfg₁ wfg₂ wfl H.
+  eapply MP.
+  2: { useBasicReasoning. apply prf_local_goals_equiv_impl_full_equiv; assumption. }
+  exact H.
+Defined.
+
+Lemma prf_local_goals_equiv_impl_full_equiv_meta_proj1 {Σ : Signature} Γ g₁ g₂ l i:
+  well_formed g₁ ->
+  well_formed g₂ ->
+  Pattern.wf l ->
+  Γ ⊢i (foldr patt_imp (g₁ <---> g₂) l) using i ->
+  Γ ⊢i (foldr patt_imp g₁ l) using i ->
+  Γ ⊢i (foldr patt_imp g₂ l) using i.
+Proof.
+  intros wfg₁ wfg₂ wfl H1 H2.
+  eapply MP.
+  2: eapply pf_iff_proj1.
+  4: apply prf_local_goals_equiv_impl_full_equiv_meta.
+  7: apply H1.
+  1: exact H2.
+  all: wf_auto2.
+Defined.
+
+Lemma prf_local_goals_equiv_impl_full_equiv_meta_proj2 {Σ : Signature} Γ g₁ g₂ l i:
+  well_formed g₁ ->
+  well_formed g₂ ->
+  Pattern.wf l ->
+  Γ ⊢i (foldr patt_imp (g₁ <---> g₂) l) using i ->
+  Γ ⊢i (foldr patt_imp g₂ l) using i ->
+  Γ ⊢i (foldr patt_imp g₁ l) using i.
+Proof.
+  intros wfg₁ wfg₂ wfl H1 H2.
+  eapply MP.
+  2: eapply pf_iff_proj2.
+  4: apply prf_local_goals_equiv_impl_full_equiv_meta.
+  7: apply H1.
+  1: exact H2.
+  all: wf_auto2.
+Defined.
+
+
+
+Lemma top_holds {Σ : Signature} Γ:
+  Γ ⊢i Top using BasicReasoning.
+Proof.
+  apply false_implies_everything.
+  { wf_auto2. }
+Defined.
+
+Lemma phi_iff_phi_top {Σ : Signature} Γ ϕ :
+  well_formed ϕ ->
+  Γ ⊢i ϕ <---> (ϕ <---> Top)
+  using BasicReasoning.
+Proof.
+  intros wfϕ.
+  toMLGoal.
+  { wf_auto2. }
+  mlSplitAnd; mlIntro.
+  - mlSplitAnd.
+    + mlIntro. mlClear 0. mlClear 0.
+      fromMLGoal.
+      apply top_holds. (* TODO: we need something like [mlExactMeta top_holds] *)
+    + fromMLGoal.
+      apply P1; wf_auto2.
+  - mlDestructAnd 0.
+    mlApply 1.
+    mlClear 0.
+    mlClear 0.
+    fromMLGoal.
+    apply top_holds.
+Defined.
+
+Lemma not_phi_iff_phi_bott {Σ : Signature} Γ ϕ :
+  well_formed ϕ ->
+  Γ ⊢i (! ϕ ) <---> (ϕ <---> ⊥)
+  using BasicReasoning.
+Proof.
+  intros wfϕ.
+  toMLGoal.
+  { wf_auto2. }
+  mlSplitAnd; mlIntro.
+  - mlSplitAnd.
+    + mlExactn 0.
+    + mlClear 0. fromMLGoal.
+      apply false_implies_everything.
+      { wf_auto2. }
+  - mlDestructAnd 0.
+    mlExactn 0.
+Defined.
+
+Lemma not_not_iff {Σ : Signature} (Γ : Theory) (A : Pattern) :
+  well_formed A ->
+  Γ ⊢i A <---> ! ! A
+  using BasicReasoning.
+Proof.
+  intros wfA.
+  apply pf_iff_split.
+  { wf_auto2. }
+  { wf_auto2. }
+  - apply not_not_intro.
+    { wf_auto2. }
+  - apply not_not_elim.
+    { wf_auto2. }
+Defined.
+
+
+Lemma patt_and_comm {Σ : Signature} Γ p q:
+  well_formed p ->
+  well_formed q ->
+  Γ ⊢i (p and q) <---> (q and p)
+  using BasicReasoning.
+Proof.
+  intros wfp wfq.
+  toMLGoal.
+  { wf_auto2. }
+  mlSplitAnd; mlIntro; mlDestructAnd 0; mlSplitAnd.
+  - mlExactn 1.
+  - mlExactn 0.
+  - mlExactn 1.
+  - mlExactn 0.
+Defined.
+
+
+
+(* We need to come up with tactics that make this easier. *)
+Local Example ex_mt {Σ : Signature} Γ ϕ₁ ϕ₂:
+  well_formed ϕ₁ ->
+  well_formed ϕ₂ ->
+  Γ ⊢i (! ϕ₁ ---> ! ϕ₂) ---> (ϕ₂ ---> ϕ₁)
+  using BasicReasoning.
+Proof.
+  intros wfϕ₁ wfϕ₂.
+  toMLGoal.
+  { wf_auto2. }
+  mlIntro. mlIntro.
+  unfold patt_not.
+  mlAssert (((ϕ₁ ---> ⊥) ---> ⊥)).
+  { wf_auto2. }
+  { mlIntro.
+    mlAssert ((ϕ₂ ---> ⊥)).
+    { wf_auto2. }
+    { mlApply 0. mlExactn 2. }
+    mlApply 3.
+    mlExactn 1.
+  }
+  mlApplyMeta (@not_not_elim Σ Γ ϕ₁ ltac:(wf_auto2)).
+  mlExactn 2.
+Defined.
+
+
+
+Local Lemma well_formed_foldr_and {Σ : Signature} (x : Pattern) (xs : list Pattern):
+  well_formed x ->
+  Pattern.wf xs ->
+  well_formed (foldr patt_and x xs).
+Proof.
+  intros wfx wfxs.
+  induction xs; simpl.
+  - assumption.
+  - feed specialize IHxs.
+    { unfold Pattern.wf in wfxs. simpl in wfxs. destruct_and!. assumption. }
+    apply well_formed_and.
+    { unfold Pattern.wf in wfxs. simpl in wfxs. destruct_and!. assumption. }
+    assumption.
+Qed.
+
+
+Lemma lhs_and_to_imp {Σ : Signature} Γ (g x : Pattern) (xs : list Pattern):
+  well_formed g ->
+  well_formed x ->
+  Pattern.wf xs ->
+  Γ ⊢i (foldr patt_and x xs ---> g) ---> (foldr patt_imp g (x :: xs))
+  using BasicReasoning.
+Proof.
+  intros wfg wfx wfxs.
+  induction xs; simpl.
+  - apply A_impl_A.
+    { wf_auto2. }
+  - pose proof (wfaxs := wfxs).
+    unfold Pattern.wf in wfxs.
+    simpl in wfxs.
+    apply andb_prop in wfxs as [wfa wfxs].
+    fold (Pattern.wf xs) in wfxs.
+    specialize (IHxs wfxs).
+    simpl in IHxs.
+    assert (Hwffa: well_formed (foldr patt_and x xs)).
+    { apply well_formed_foldr_and; assumption. }
+    toMLGoal.
+    { wf_auto2. }
+    do 3 mlIntro.
+    mlAdd IHxs.
+    mlAssert (((foldr patt_and x xs ---> g) ---> foldr patt_imp g xs)).
+    { wf_auto2. }
+    { mlIntro.
+      mlAssert ((x ---> foldr patt_imp g xs)).
+      { wf_auto2. }
+      { mlApply 0. mlExactn 4. }
+      mlClear 0.
+      mlApply 4.
+      mlExactn 1.
+    }
+    mlClear 0.
+    mlApply 3.
+    mlClear 3.
+    mlIntro.
+    mlApply 0.
+    mlSplitAnd.
+    + mlExactn 2.
+    + mlExactn 3.
+Defined.
+
+Lemma lhs_and_to_imp_meta {Σ : Signature} Γ (g x : Pattern) (xs : list Pattern) i:
+  well_formed g ->
+  well_formed x ->
+  Pattern.wf xs ->
+  Γ ⊢i (foldr patt_and x xs ---> g) using i ->
+  Γ ⊢i (foldr patt_imp g (x :: xs)) using i.
+Proof.
+  intros wfg wfx wfxs H.
+  eapply MP.
+  2: { useBasicReasoning. apply lhs_and_to_imp; assumption. }
+  exact H.
+Defined.
+
+
+
+
+#[local]
+Ltac tryExact l idx :=
+  match l with
+    | nil => idtac
+    | (?a :: ?m) => try mlExactn idx; tryExact m (idx + 1)
+  end.
+
+#[global]
+Ltac mlAssumption :=
+  match goal with
+    | [ |- @of_MLGoal ?Sgm (@mkMLGoal ?Sgm ?Ctx ?l ?g ?i) ] 
+      =>
+        tryExact l 0
+  end.
+
+
+
+
+  Lemma impl_eq_or {Σ : Signature} Γ a b:
+  well_formed a ->
+  well_formed b ->
+  Γ ⊢i ( (a ---> b) <---> ((! a) or b) )
+  using BasicReasoning.
+Proof.
+  intros wfa wfb.
+  toMLGoal.
+  { wf_auto2. }
+  repeat mlIntro.
+  mlDestructOr 0.
+  - mlApply 0. mlIntro. mlClear 0. mlIntro.
+    mlApplyMeta (@not_not_elim _ _ _ _) in 1.
+    mlApply 0. mlAssumption.
+  - mlApply 0. mlIntro. mlClear 0. mlIntro.
+    mlDestructOr 0.
+    + mlApplyMeta (@false_implies_everything _ _ _ _).
+      mlApply 0. mlAssumption.
+    + mlAssumption.
+  Unshelve. all: assumption.
+Qed.
+
+
+Lemma nimpl_eq_and {Σ : Signature} Γ a b:
+  well_formed a ->
+  well_formed b ->
+  Γ ⊢i ( ! (a ---> b) <---> (a and !b) )
+  using BasicReasoning.
+Proof.
+  intros wfa wfb.
+  toMLGoal.
+  { wf_auto2. }
+  repeat mlIntro.
+  mlDestructOr 0.
+  - mlApply 0. repeat mlIntro.
+    mlApply 1. mlIntro.
+    mlDestructOr 2.
+    + mlApplyMeta (false_implies_everything _ _).
+      mlApply 2. mlAssumption.
+    + mlApplyMeta (@not_not_elim _ _ _ _) in 2.
+      mlAssumption.
+  - mlApply 0. repeat mlIntro.
+    mlDestructAnd 1. mlApply 2. mlApply 3.
+    mlAssumption.
+  Unshelve. all: assumption.
+Qed.
+
+
+Lemma deMorgan_nand {Σ : Signature} Γ a b:
+    well_formed a ->
+    well_formed b ->
+    Γ ⊢i ( !(a and b) <---> (!a or !b) )
+    using BasicReasoning.
+  Proof.
+    intros wfa wfb.
+    toMLGoal.
+    { wf_auto2. }
+    repeat mlIntro.
+    mlDestructOr 0.
+    - mlRevert. mlApplyMeta (@not_not_intro _ _ _ _). repeat mlIntro.
+      mlApplyMeta (@not_not_elim _ _ _ _) in 1.
+      mlApply 0. mlIntro.
+      mlDestructOr 3.
+      all: mlApply 3; mlAssumption.
+    - mlRevert. mlApplyMeta (@not_not_intro _ _ _ _). repeat mlIntro.
+      mlDestructAnd 1.
+      mlDestructOr 0.
+      all: mlApply 0; mlAssumption.
+    Unshelve. all: auto.
+  Qed.
+
+Lemma deMorgan_nor {Σ : Signature} Γ a b:
+    well_formed a ->
+    well_formed b ->
+    Γ ⊢i ( !(a or b) <---> (!a and !b))
+    using BasicReasoning.
+  Proof.
+    intros wfa wfb.
+    toMLGoal.
+    { wf_auto2. }
+    repeat mlIntro.
+    mlDestructOr 0.
+    - mlRevert. mlApplyMeta (@not_not_intro _ _ _ _). repeat mlIntro.
+      mlApply 0.
+      mlDestructOr 1.
+      + mlApplyMeta (@not_not_elim _ _ _ _) in 1.
+        mlLeft. mlAssumption.
+      + mlApplyMeta (@not_not_elim _ _ _ _) in 1.
+        mlRight. mlAssumption.
+    - mlRevert. mlApplyMeta (@not_not_intro _ _ _ _). repeat mlIntro.
+      mlDestructAnd 0.
+      mlDestructOr 2.
+      + mlApply 0. mlAssumption.
+      + mlApply 1. mlAssumption.
+    Unshelve. all: wf_auto2.
+  Qed.
+
+Lemma not_not_eq {Σ : Signature} (Γ : Theory) (a : Pattern) :
+  well_formed a ->
+  Γ ⊢i (!(!a) <---> a)
+  using BasicReasoning.
+Proof.
+  intros wfa.
+  toMLGoal.
+  { wf_auto2. }
+  mlIntro.
+  mlDestructOr 0.
+  - mlApply 0. mlIntro.
+    mlApplyMeta (@not_not_elim _ _ _ _) in 1.
+    mlAssumption.
+  - unfold patt_not. mlApply 0. repeat mlIntro.
+    mlApply 2. mlAssumption.
+  Unshelve.
+  all: assumption.
+Defined.
+
+
+(**********************************************************************************)
+
+
+
+
+(* This is an example and belongs to the end of this file.
+   Its only purpose is only to show as many tactics as possible.\
+ *)
+ Example ex_and_of_equiv_is_equiv_2 {Σ : Signature} Γ p q p' q' i:
+ well_formed p ->
+ well_formed q ->
+ well_formed p' ->
+ well_formed q' ->
+ Γ ⊢i (p <---> p') using i ->
+ Γ ⊢i (q <---> q') using i ->
+ Γ ⊢i ((p and q) <---> (p' and q')) using i.
+Proof.
+ intros wfp wfq wfp' wfq' pep' qeq'.
+ pose proof (pip' := pep'). apply pf_conj_elim_l_meta in pip'; auto.
+ pose proof (p'ip := pep'). apply pf_conj_elim_r_meta in p'ip; auto.
+ pose proof (qiq' := qeq'). apply pf_conj_elim_l_meta in qiq'; auto.
+ pose proof (q'iq := qeq'). apply pf_conj_elim_r_meta in q'iq; auto.
+
+ toMLGoal.
+ { wf_auto2. }
+ unfold patt_iff.
+ mlSplitAnd.
+ - mlIntro.
+   mlDestructAnd 0.
+   mlSplitAnd.
+   + mlApplyMeta pip'.
+     mlExactn 0.
+   + mlApplyMeta qiq' in 1.
+     mlExactn 1.
+ - mlIntro.
+   unfold patt_and at 2.
+   unfold patt_not at 1.
+   mlIntro.
+   mlDestructOr 1.
+   + mlDestructAnd 0.
+     unfold patt_not.
+     mlApply 2.
+     mlClear 2.
+     mlClear 1.
+     fromMLGoal.
+     exact p'ip.
+   + mlAdd q'iq.
+     mlDestructAnd 1.
+     mlAssert (q).
+     { wf_auto2. }
+     { mlApply 0. mlExactn 2. }
+     unfold patt_not at 1.
+     mlApply 3.
+     mlExactn 4.
+Defined.
+
+
+#[local]
+  Example ex_or_of_equiv_is_equiv_2 {Σ : Signature} Γ p q p' q' i:
+    well_formed p ->
+    well_formed q ->
+    well_formed p' ->
+    well_formed q' ->
+    Γ ⊢i (p <---> p') using i ->
+    Γ ⊢i (q <---> q') using i ->
+    Γ ⊢i ((p or q) <---> (p' or q')) using i.
+  Proof.
+    intros wfp wfq wfp' wfq' pep' qeq'.
+
+    pose proof (pip' := pep'). apply pf_conj_elim_l_meta in pip'; auto.
+    pose proof (p'ip := pep'). apply pf_conj_elim_r_meta in p'ip; auto.
+    pose proof (qiq' := qeq'). apply pf_conj_elim_l_meta in qiq'; auto.
+    pose proof (q'iq := qeq'). apply pf_conj_elim_r_meta in q'iq; auto.
+
+    toMLGoal.
+    { wf_auto2. }
+    unfold patt_iff.
+    mlSplitAnd.
+    - mlIntro.
+      mlDestructOr 0.
+      mlLeft.
+      + mlApplyMeta pip'.
+        mlExactn 0.
+      + mlRight.
+        mlApplyMeta qiq'.
+        mlExactn 0.
+    - mlIntro.
+      mlDestructOr 0.
+      mlLeft.
+      + mlApplyMeta p'ip.
+        mlExactn 0.
+      + mlRight.
+        mlApplyMeta q'iq.
+        mlExactn 0. 
+  Defined.
